$$\displaylines{
(x^{ 2 }-x)\cdot e^{ -x } \\
e^{ -x } = g_{ 1 }(-x) = \sum_{k=0}^{n} \frac{(-1)^{ k }x^{ k }}{k!} + o(x^{ n }) \\
\sum_{k=0}^{n} \frac{(-1)^{ k }x^{ k +2}}{k!} -\sum_{k=1}^{n} \frac{(-1)^{ k }x^{ k+1 }}{k!} + o(x^{ n+1 })\\
-x\sum_{k=0}^{n} \frac{(-1)^{ k }x^{ k+2 }}{k!} - \sum_{m=0}^{n-1} \frac{(-1)^{ m+1 }x^{ m+2 }}{(m+1)!} + o(x^{ n +1}) \\
-x+\sum_{k=0}^{n-1} \left( \frac{(-1)^{ k }}{k!} + \frac{(-1)^{ m }}{(m+1)!} \right)x^{ k+2 }+o(x^{ n+1 }) \\
-x + \sum_{m=2}^{n} \left( \frac{(-1)^{ n-2 }}{(n-2)!} + \dfrac{(-1)^{ m-2 }}{(n-1)!} \right) x^{ m }+o(x^{ n })
}$$
### Разложение по формуле Тейлора.
Уровень 5.

$$\displaylines{
y = f(x) \text{ до } o(x^{ n }) \\
\text{ где } f'(x) = \sum_{k=0}^{n} a_{ k }x^{ k } + o(x^{ n }) \\
\text{ Метод: } f(x) = f(0) + \sum_{k=0}^{n} a_{ k } \dfrac{x^{ k+1 }}{k+1} + o(x^{ n+1 }) 
}$$
Пример.
$$\displaylines{
y = \arctan{(x)} \quad o(x^{ n }) \\
y' = \frac{1}{1+x^{ 2 }} = g_{ 6 }(x^{ 2 }) = \sum_{k=0}^{n}(-1)^{ k } x^{ 2k } + o(x^{ 2n }) \\
\arctan{(x)} = \sum_{k=0}^{n} \dfrac{(-1)^{ n }x^{ 2k+1 }}{2k+1} + o(x^{ 2n+1 }) = x-\frac{x^{ 3 }}{3}+\frac{x^{ 5 }}{5}-\frac{x^{ 7 }}{7}+\frac{x^{ 9 }}{9}  
}$$
Зам.
$$\displaylines{
y = f(x) \quad x = x_{ 0 } \neq  0 \\
n = n_{0} \\
\text{ Разложить до  }o(x-x_{ 0 })^{ n } \\
\text{ Замена. } t = x-x_{ 0 } \\
x = t+x_{ 0 } \\
f(t) = \dots = \sum_{k=0}^{n} a_{ k }t^{ k } + o(t^{ n }) \\
f(x-x_{ 0 }) = \sum_{k=0}^{n} a_{ k }(x-x_{ 0 })^{ n } + o(x-x_{ 0 }) ^{ n }
}$$
Пример.
$$\displaylines{
f(x) = \frac{1}{x} \quad x_{ 0 } = 2 \quad o(x-2)^{ n } \\
\text{ Замена } t = x-2 \\
x = t+2 \\
\implies f(t) = \frac{1}{t+2} =\frac{1}{2} \cdot \frac{1}{1+\frac{t}{2}} = \frac{1}{2}g_{ 6 }\left( \frac{t}{2} \right) = \frac{1}{2} \sum_{k=0}^{n} \dfrac{(-1)^{ k }t^{ k }}{2^{ k }} + o(t^{ n })  = \sum_{k=0}^{n} \frac{(-1)^{ k }(x-2)^{ k }}{2^{ k+1 }} + o(x-2)^{ n }
}$$

### Раскрытие неопределенности с помощью формулы Тейлора.
Основа.

Утв.
$$\displaylines{
\lim_{ x \to 0 } \dfrac{ax^{ n } +o(x^{ n })}{bx^{ n }+o(x^{ n })} = \begin{cases}
\dfrac{a}{b} &  a, \ b\neq 0  \\
0   & a = 0, \  b \neq 0 \\
\infty & a\neq  0, \  b = 0  \\
\left[\dfrac{0}{0} \right] & a = b = 0 
\end{cases}
}$$
Пример.
$$\displaylines{
\lim_{ x \to 0 } {\dfrac{\tan{(x)}-\sin{(x)}}{x^{ 3 }} } = \lim_{ x \to 0 } {\dfrac{x+\frac{x^{ 3 }}{3}+o(x^{ 3 }) -\left( x-\frac{x^{ 3 }}{6}+o(x^{ 3 }) \right)} {x^{ 3 } }} = \lim_{ x \to 0 } {\dfrac{\frac{1}{2}x^{ 3 }+o(x^{ 3 })}{x^{ 3 }} } = \frac{1}{2} 
}$$
Пример.
$$\displaylines{
\lim_{ x \to 0 } {\dfrac{\sqrt[5]{ 1+2x }-1}{\sqrt[4]{ 1+x }-\sqrt{ 1-x }} } = \left[ \frac{0}{0}  \right] = \lim_{ x \to 0 } {\frac{\frac{1}{5}\cdot 2x}{1+\frac{1}{4}x + o(x) - \left( 1-\frac{1}{2}x+o(x) \right)} } = \frac{\frac{2}{5}x}{\frac{3}{4}x+o(x)} = \frac{8}{15}  
}$$
Пример.
$$\displaylines{
\lim_{ x \to 0 } {\frac{\sqrt{ 1+2\tan{(x)} }-e^{ x }+x^{ 2 }}{\arcsin{(x)}-\sin{(x)}} } \\
1. \text{ Знаменатель } x+\frac{x^{ 3 }}{6}+o(x^{ 3 }) \\
-\left( x-\frac{x^{ 3 }}{6} + o(x^{ 3 }) \right) = \frac{x^{ 3 }}{3} + o(x^{ 3 }) 
}$$
$$\displaylines{
(1+2\tan{(x)})^{ 1/2 } = g_{ 4 }(2\tan{(x)}) = 1+\tan{(x)} -\frac{1}{2}\tan{(x)} + \frac{\frac{1}{2}\left( -\frac{1}{2} \right)\left( -\frac{3}{2} \right)}{6} \cdot 8\tan{(x)}^{ 3 } + o(\tan{(x)}^{ 3 }) = 1+\left( x+\frac{x^{ 3 }}{3} \right) - \frac{1}{2}\left( x+\frac{x^{ 3 }}{3} \right)^{ 2 } + \frac{1}{2}\left( x+\frac{x^{ 3 }}{3} \right)^{ 3 } + o(x^{ 3 }) = \\
= 1+ x + \frac{x^{ 3 }}{3} -\frac{1}{2}x^{ 2 }+\frac{1}{2}x^{ 3 }+o(x^{ 3 }) \\ \\
= \lim_{ x \to 0 } {\frac{1+x-\frac{1}{2}x^{ 2 }+\frac{5}{6}x^{ 3 }-\left( 1+x+\frac{x^{ 2 }}{2}+\frac{x^{ 3 }}{6} \right)+x^{ 2 }+o(x^{ 3 })}{\frac{x^{ 3 }}{3}+o(x^{ 3 })} } = 2
}$$