$$\displaylines{
\frac{C_{ n }^{ k }}{k + 1} = \frac{n \cdot (n - 1) \dots (n - k + 1)}{1 \cdot 2 \dots k(k + 1)} = \frac{(n + 1)n(n - 1)\dots(n - k + 1)}{(k + 1)! \cdot (n +  1)} = \frac{C_{ n + 1}^{ k + 1 }}{n + 1} \\ 
}$$

# Binomial Theorem 
$$\displaylines{
1. \ \ C_{ n }^{ 0 } = C_{ n }^{ n } = 1 \\ 
2. \ \ C_{ n }^{ k } = C_{ n }^{ k - 1 } \\ 
3. \ \ C_{ n }^{ k } + C_{ n }^{ k + 1 } = C_{ n + 1 }^{ k + 1 } \\ 
C_{ n }^{ k } + C_{ n }^{ k + 1 } = C_{ n + 1 }^{ k + 1 } \\ 
\frac{n!}{(n - k)! \cdot k!} + \frac{n!}{(n - k - 1)! \cdot (k + 1)!} = \\ 
= \frac{n!}{(n - k - 1)! \cdot (n - k) \cdot k!} + \frac{n!}{(n - k - 1)! \cdot k! \cdot (k + 1)} = \\
= \frac{n!}{(n - k - 1)! \cdot k!} \cdot \left( \frac{1}{n - k} + \frac{1}{k + 1} \right) = \\ 
= \frac{n!}{(n - k - 1)! \cdot k!} \cdot \left( \frac{ 1 + n }{(n - k)(k + 1)} \right) = \\ 
= \frac{n! \cdot (n + 1)}{(n - k - 1)! \cdot (n - k) \cdot k! (k + 1)} = \frac{(n + 1)!}{(n - k)! \cdot (k + 1)!} = C_{ n + 1 }^{ k + 1 } 
}$$

$$\displaylines{
(a + b)^{ 6 } = a^{ 6 } + 6 \cdot a^{ 5 } \cdot b + 15 \cdot a^{ 4 } \cdot b^{2} + 20 \cdot a^{ 3 } \cdot b^{ 3 } + 15 \cdot a^{ 4 } \cdot b^{2} + 6 \cdot a^{ 5 } \cdot b + b^{ 6 }
}$$

$$\displaylines{
\left( \sqrt{ x } + \frac{1}{\sqrt[3]{ x }} \right)^{ 16 } \\ 
\text{Найти член разложения с } x^{ 3 } \\ 
C_{ 16 }^{ k } (\sqrt{ x })^{ k } \cdot \left( \frac{1}{\sqrt[3]{ x }} \right)
}$$