**Решить заново:**
$$\displaylines{
\lim_{ n \to \infty } \left( \frac{n + 10}{2n - 1} \right)^{ n } = 0^{ \infty } = 0
}$$

# Техника Раскрытия Неопределенностей
## Уровень 5 (ОЛТ) 
**Основа:**
$$\displaylines{
x = e^{ \ln(x) } \\ 
x^{ y } = e^{ \lg(x)^{ y } } = e^{ y \cdot \ln(x) }
}$$


**Тип 5.1:** 
$$\displaylines{
\lim_{ n \to \infty } x_{ n }^{ y_{ n } } = [\infty^{ 0 }, 0^{ 0 }] = \lim_{ n \to \infty } e^{ y_{ n } \cdot \ln(x_{ n }) }
}$$

Пример 1: 
$$\displaylines{
\lim_{ n \to \infty } \sqrt[n]{ n } = \lim_{ n \to \infty } n^{ \frac{1}{n} } = \infty^{ 0 } = (*) \\ 
(*) = \lim_{ n \to \infty } e^{ \ln\left( n^{ \frac{1}{n} } \right) } = \lim_{ n \to \infty } e^{ \frac{1}{n} \cdot \ln(n) } = e^{ 0 } = 1
}$$

Пример 2: 
$$\displaylines{
\lim_{ n \to \infty } \left( \frac{1}{3^{ n } + n} \right)^{ \frac{1}{n + 2} } = 0^{ 0 } = (*) \\ 
(*) = \lim_{ n \to \infty } e^{ \frac{1}{n + 2} \cdot \ln\left( \frac{1}{3^{ n } + n} \right) } = \lim_{ n \to \infty } e^{ \frac{-\ln\left( 3^{ n } + n \right)}{n + 2} } = \lim_{ n \to \infty } e^{ \frac{-\ln(3^{ n })}{n + 2} } = \lim_{ n \to \infty } e^{ \frac{-n \cdot \ln(3)}{n} } = \frac{1}{3}
}$$

Пример 3: 
$$\displaylines{
\lim_{ n \to \infty } (n + 1)^{ \frac{2}{\ln(n) + 3} } = \infty^{ 0 } = (*) \\ 
\begin{aligned}
(*) &= \lim_{ n \to \infty } e^{ \frac{2}{\ln(n) + 3}  \cdot \ln(n + 1)} \\ 
&= \lim_{ n \to \infty } e^{ \frac{2 \cdot \ln(n + 1)}{\ln(n) + 3} } \\ 
&= \lim_{ n \to \infty } e^{ \frac{2 \cdot \ln(n)}{\ln(n)} } \\ 
&= e^{ 2 }
\end{aligned}
}$$

# Теорема В. 
**Пример:**
$$\displaylines{
\text{Последовательность: }
x_{ n } = \left( 1 - \frac{1}{2^{2}} \right), \left( 1 - \frac{1}{3^{2}} \right), \dots, \left( 1 - \frac{1}{n^{2}} \right), \left( 1 - \frac{1}{(n + 1)^{2}} \right) \\ 
\text{Доказать сходимость: }  1 - \frac{1}{((n + 1) + 1)^{2}} \\ 
\frac{x_{ n + 1 }}{x_{ n }} = 1 - \frac{1}{(n + 2)^{2}} < 1 \\ 
x_{ n + 1 } < x_{ n } \implies \begin{matrix}x_{ n } \downarrow \\ x_{ n } \geq 0\end{matrix} \implies x_{ n } \text{ – сход. (теорема В.)}
}$$

**Двойной Факториал.**

Пример: 
$$\displaylines{
x_{ n } = \frac{(2n - 1)!!}{2n!!} = \frac{1 \cdot 3 \cdot 5 \dots (2n - 1)}{2 \cdot 4 \cdot 6\dots(2n)} \\ 
\frac{x_{ n + 1 }}{x_{ n }} = \frac{1 \cdot \dots \cdot (2n + 1) \cdot 2 \cdot 2n}{2 \cdot \dots \cdot (2n + 2) \cdot 1 \cdot \dots \cdot (2n - 1)} = \frac{2n + 1}{2n + 2} = 1 -\frac{1}{2n + 2} < 1 \implies \\
\implies x_{ n + 1 } < x_{ n } \implies \begin{matrix}x_{ n } \downarrow \\ x_{ n } \geq 0\end{matrix} \implies x_{ n } \text{ – сход.} \\ 
\text{Пример: } \frac{x_{ 3 }}{x_{ 2 }} = \frac{1 \cdot 3 \cdot 5}{2 \cdot 4 \cdot 6} : \frac{1 \cdot 3}{2 \cdot 4} = \frac{1 \cdot 3 \cdot 5 \cdot 2 \cdot 4}{2 \cdot 4 \cdot 6 \cdot 1 \cdot 3}
}$$

**Замечание:** 
$$\displaylines{
x_{ n + 1 } = \frac{x_{ n + 1 }}{x_{ n }} \cdot x_{ n }
}$$

Пример: Доказать сходимость и вычеслить предел.
$$\displaylines{
x_{ n } = \frac{n^{2}}{5^{ n }} \\ 
\frac{x_{ n  + 1}}{x_{ n }} = \frac{(n + 1)^{2} \cdot 5^{ n }}{(5^{ n + 1 }) \cdot n^{2}} = \left( 1 + \frac{1}{n} \right)^{2} \cdot \frac{1}{5} \leq \frac{4}{5} < 1 \implies \begin{matrix}x_{ n } \downarrow \\ x_{ n } > 0 \end{matrix} \implies x_{ n } \text{ – сходится} \\ 
\underset{ \to a }{ x_{ n + 1} } = \underset{ \frac{1}{5} }{ \left( 1 + \frac{1}{n} \right)^{2} \cdot \frac{1}{5} } \cdot \underset{ \to a }{ x_{ n } } 
}$$

# Критерий Коши
**Критерий Коши:**
$$\displaylines{
\{ x_{ n } \text{ – сходится} \} \Leftrightarrow \{ \forall \epsilon > 0 \ \ \exists N \in N \ \ \forall n > N \ \ \forall p \in \mathbb{N} \implies |x_{ n + p } - x_{ n }| < \epsilon \}
}$$

Пример: 
$$\displaylines{
x_{ n } = 1 + \frac{1}{2} + \frac{1}{3} + \frac{1}{4} + \dots + \frac{1}{2^{ n } + 1} \\ 
\text{Первый пункт:} \\ 
|x_{ n + p } - x_{ n }| = |1 + \frac{1}{2} + \dots + \frac{1}{2^{ n + p - 1 }} - \left( \frac{1}{2} + \dots + \frac{1}{2^{ n - 1 }} \right)| = \underset{ \text{p слагаемых} }{ \frac{1}{2} + \dots + \frac{1}{2^{ n + p - 1 }} } = \frac{1}{2^{ n }} \cdot \frac{1 - \left( \frac{1}{2} \right)^{ p }}{1 - \frac{1}{2}} = \\ 
= \frac{1}{2^{ n - 1 }} \cdot \left( 1 - \frac{1}{2^{ p }} \right) \leq \frac{1}{2^{ n - 1 }} \leq \frac{1}{n} \\ 
\text{Второй пункт:} \\ 
2^{ n - 1 } \geq n \\ 
1. \ \ \frac{1}{n} < \epsilon \\ 
2. \ \ N(\epsilon) = \left[ \frac{1}{\epsilon} \right] + 1 \\ 
}$$

Пример: Доказать по КК. 
$$\displaylines{
x_{ n } = \frac{\sin \alpha}{3} + \frac{\sin 2\alpha}{3^{2}} + \dots + \frac{\sin n\alpha}{3^{ n }} \\ 
|x_{ n + p} x_{ n }| = | \frac{\sin(n + 1)\alpha}{3^{ n + 1 }} + \dots + \frac{\sin(n + p)\alpha}{3^{ n + p }}| \leq | \frac{\sin(n + 1)\alpha}{3^{ n } + 1}| + \dots + | \frac{\sin(n + p)}{3^{ n } + p}| \leq \frac{1}{3^{ n + 1 }} + \dots + \frac{1}{3^{ n + p }} = \frac{1}{3^{ n + 1 }} \cdot \frac{1 - \left( \frac{1}{3} \right)^{ p }}{1 - \frac{1}{3}} = \frac{1}{3^{ n }  \cdot 2} \cdot \left( 1 - \frac{1}{3^{ n }} \right)  \leq \frac{1}{3^{ n } \cdot 2} \leq \frac{1}{2n} < \epsilon \\ 
\frac{1}{2n}
}$$