$$\displaylines{
\text{ Быстрая часть }\begin{cases}
e^x = 1 + x + \frac{x^2}{2!} + \frac{x^3}{3!} + \frac{x^4}{4!} + \dots + \frac{x^n}{n!} + o(x^n) \\ \\
\sin(x) = x - \frac{x^3}{3!} + \frac{x^5}{5!} - \dots + (-1)^n \frac{x^{2n+1}}{(2n+1)!} + o(x^{2n+1}) \\ \\
\cos(x) = 1 - \frac{x^2}{2!} + \frac{x^4}{4!} - \dots + (-1)^n \frac{x^{2n}}{(2n)!} + o(x^{2n}) \\
\end{cases} \\ \\ \text{ Медленная часть }
\begin{cases}
\ln(1+x) = x - \frac{x^2}{2} + \frac{x^3}{3} - \frac{x^4}{4} + \dots + (-1)^{n+1} \frac{x^n}{n} + o(x^n) \\ \\
\arctan(x) = x - \frac{x^3}{3} + \frac{x^5}{5} - \dots + (-1)^n \frac{x^{2n+1}}{2n+1} + o(x^{2n+1}) \\
\end{cases} \\ \\
\frac{1}{1-x} = 1 + x + x^2 + x^3 + \dots + x^n + o(x^n) \\
\frac{1}{1+x} = 1 - x + x^2 - x^3 + \dots + (-1)^n x^n + o(x^n) \\
(1+x)^a = 1 + ax + \frac{a(a-1)}{2}x^2 + \frac{a(a-1)(a-2)}{6}x^3 + \dots + \frac{a(a-1)\dots(a-n+1)}{n!}x^n + o(x^n) \\
\sinh(x) = x + \frac{x^3}{3!} + \frac{x^5}{5!} + \dots + \frac{x^{2n+1}}{(2n+1)!} + o(x^{2n+1}) \\
\cosh(x) = 1 + \frac{x^2}{2!} + \frac{x^4}{4!} + \dots + \frac{x^{2n}}{(2n)!} + o(x^{2n})
}$$
