1 вариант.
$$\displaylines{
\begin{aligned}
&\  \begin{aligned}\text{i}.
\int \frac{(\sqrt{ x } + \sqrt[3]{ x })^{ 2 }}{x^{ 2 }}  \, dx  &= \int_{}^{} \left( \frac{x}{x^{ 2 }} + \frac{2x^{ 5/6 }}{x^{ 2 }} + \frac{x^{ 2/3 }}{x^{ 2 }} \right)  \, dx =  \\& =  \int_{}^{} (x^{ -1 } + 2x^{ -7/6 } + x^{ -4/3 }) \, dx = \ln|x| - 12x^{ -1/6 } - 3 x^{ -1/3 } + C
\end{aligned} \\
& \begin{aligned}\text{ ii. }\
\int_{0}^{\pi/3} e^{ x }\sin{(x)} \, dx &= \frac{e^{ x }}{2}\big[\sin{(x)} - \cos{(x)}\big] \bigg|_{ 0 }^{ \pi/3 } = \\ & = \frac{e^{ \pi/3 }}{2}\left( \sin{\left( \frac{\pi}{3}  \right)} - \cos{\left( \frac{\pi}{3} \right)} \right) - \frac{e^{ 0 }}{2}(\sin{(0)} - \cos{(0)}) = \\ & = \frac{e^{ \pi/3 }}{2}\left( \frac{\sqrt{ 3 }}{2} - \frac{1}{2} \right) + \frac{1}{2}
\end{aligned}
\end{aligned}
}$$

2 вариант.
$$\displaylines{
\begin{aligned}
& \ \begin{aligned}\text{i}.\int \frac{\sqrt[3]{ x }}{1 + \sqrt[3]{ x }}  \, dx &= \begin{vmatrix}
t = \sqrt[3]{ x }  \\
x = t^{ 3 } & dx = 3t^{ 2 }
\end{vmatrix} = 
\int_{}^{} \frac{3t^{ 3 }}{t + 1} \, dt = \\ & = \int_{}^{} \left( 3t^{ 2 } - 3t + 3 - \frac{3}{t + 1} \right) \, dt = \\ & =  t^{ 3 } - \frac{3}{2}t^{ 2 } + 3t - 3\ln|t+1| + C = \\ & =  x - \frac{3}{2}x^{ 2/3 } + 3x^{ 1/3 } - 3 \ln|x^{ 1/3 } + 1| + C
\end{aligned} \\
&\text{ ii. }\ \int_{1}^{e} x^{ 2 }\ln(x) \, dx = \frac{1}{3}x^{ 3 } \ln(x) - \frac{1}{9}x^{ 3 } \bigg|_{ 1 }^{ e } = \frac{1}{9}(2e^{ 3 } + 1)
\end{aligned}
}$$

3 вариант.
$$\displaylines{
\begin{aligned}
&\text{i}. \ \int \frac{1}{\sqrt{ e^{ x }-4 }} \, dx = \int_{}^{} \frac{1}{t} \cdot  \frac{2t}{t^{ 2 } - 4} \, dt = \arctan{\left( \frac{\sqrt{ e^{ x }-4 }}{2} \right)} + C \\
&\text{ ii. }\ \int_{0}^{1} \left( \sqrt{ x } + \sqrt[3]{ x^{ 2 } } + \frac{1}{x+1} \right) \, dx  = \left[  \frac{2}{3}x^{ 3/2 } + \frac{3}{5}x^{ 5/3 } + \ln|x+1| \right]_{ 0 }^{ 1 } = \frac{19}{15} + \ln(2)
\end{aligned}
}$$

4 вариант.
$$\displaylines{
\begin{aligned}
&\text{i}. \ \int e^{ x }(x^{ 2 } + 3x - 1) \, dx = e^{ x } (x^{ 2 } + 3x - 1) - e^{ x }(2x+3) + 2e^{ x } + C \\
&\text{ ii. }\ \int_{0}^{\sqrt{ 3 }} \frac{x}{\sqrt{ 4-x^{ 2 } }} \, dx = \begin{vmatrix}
t = 4-x^{ 2 }\\
dt = -2xdx \\
xdx = -\frac{dt}{2}
\end{vmatrix} = \frac{1}{2}\int_{1}^{4} \frac{1}{\sqrt{ t }} \, dt = \sqrt{ t }\bigg|_{ 1 }^{ 4 } = \sqrt{ 4 } - \sqrt{ 1 } = 1
\end{aligned}
}$$

5 вариант.
$$\displaylines{
\begin{aligned}
&\text{i}. \ \int \frac{5x-4}{(x-2)(x+1)}  \, dx = \int_{}^{} \frac{2}{x-2} + \frac{3}{x+1} \, dx  = 2\ln|x-2| + 3\ln|x+1| + C\\
&\text{ ii. }\ \int_{1}^{4} \frac{2e^{ \sqrt{ x } }+3}{\sqrt{ x }} \, dx = \int_{1}^{4} \frac{2e^{ \sqrt{ x } }}{\sqrt{ x }} \, dx + \int_{1}^{4} \frac{3}{\sqrt{ x }} \, dx  =4e^{ t } \bigg|_{ 1 }^{ 2 } + 6\sqrt{ x } \bigg|_{ 1 }^{ 4 } = 4(e^{ 2 } - e) + 6
\end{aligned}
}$$
6 вариант.
$$\displaylines{
\begin{aligned}
& \ \begin{aligned}\text{i}. \ 
\int \frac{4x-5}{x^{ 2 } -4x+13} \, dx & = 2\int_{}^{} \frac{2x - 4 }{x^{ 2 } - 4x + 13} \, dx  + 3\int_{}^{} \frac{1}{x^{ 2 } - 4x + 13} \, dx = \\ & =  2\ln|x^{ 2 } - 4x + 13| + 3 \int_{}^{} \frac{1}{(x-2)^{ 2 } + 9} \, dx = \\ & = 2\ln|x^{ 2 } - 4x + 13| + \arctan{\left( \frac{x-2}{3} \right)} + C
\end{aligned}\\
&\text{ ii. }\ \int_{0}^{1} \sqrt[3]{ (x^{ 5 } + 2)^{ 2 } }x^{ 4 } \, dx = \begin{vmatrix}
t = x^{ 5 } + 2 \\
dt = 5x^{ 4 }dx \\
x^{ 4 }dx = \frac{dt}{5}
\end{vmatrix} = \frac{1}{5}\int_{2}^{3} t^{ 2/3 } \, dt = \frac{3}{25}t^{ 5/3 } \bigg|_{ 2 }^{ 3 } = \frac{3}{25}(3^{ 5/3 } - 2^{ 5/3 })
\end{aligned}
}$$

7 вариант.
$$\displaylines{
\begin{aligned}
&\text{i}. \ \int \frac{1}{4 + \sqrt{ x }}  \, dx = \begin{vmatrix}
t = \sqrt{ x } \\
t^{ 2 } = x \\
dx = 2tdt
\end{vmatrix} = 2\int_{}^{} \frac{t}{t + 4} \, dt = 2 \int_{}^{} 1 - \frac{4}{t+4} \, dt = 2\sqrt{ x } - 8\ln|\sqrt{ x } + 4| + C\\
&\text{ ii. }\ \int_{1}^{e} \frac{1}{x(\ln(x)^{ 2 } - 4)}  \, dx = \begin{vmatrix}
t = \ln(x) \\
dt = \frac{dx}{x}
\end{vmatrix} = \int_{0}^{1} \frac{1}{t^{ 2 } -4} \, dt = \frac{1}{4}\ln\left| \frac{t-2}{t+2} \right| \bigg|_{ 0 }^{ 1 } = \frac{1}{4} \ln \frac{1}{3} = -\frac{1}{4}\ln3  
\end{aligned}
}$$

8 вариант.
$$\displaylines{
\begin{aligned}
&\text{i}. \ \int \frac{x^{ 3 } + 2x^{ 2 } - x + 1}{x+2} \, dx = \int_{}^{} \left( x^{ 2 } - 1 + \frac{3}{x+2} \right) \, dx  = \frac{1}{3}x^{ 3 } - x + 3\ln|x+2| + C\\
& \begin{aligned}\text{ ii. }\
\int_{6}^{12} \left( 2\sqrt[3]{ x-4 } - \frac{1}{\sqrt[3]{ x-4 }} \right) \, dx &= \begin{vmatrix}
t = x-4 \\
dt = dx
\end{vmatrix} = \int_{2}^{8} 2t^{ 1/3 } - t^{ -1/3 } \, dt = \frac{3}{2}\left[ t^{ 4/3 }-t^{ 2/3 } \right]_{ 2 }^{ 8 } = \\
& = \frac{3}{2}\left(  8^{ 4/3 } - 8^{ 2/3 } \right) - \frac{3}{2}\left(  2^{ 4/3 } -  2^{ 2/3 } \right) = 18  - \frac{3}{2} ( 2^{ 4/3  } + 2^{ 2/3 })
\end{aligned}
\end{aligned}
}$$
