Пример:
$$\displaylines{
\int \frac{dx}{\sqrt[3]{ \sin{(x)^{ 5 } \cos{(x)}} }} = \int \frac{dx}{\sqrt[3]{ \dfrac{\sin{(x)}^{ 5 }}{\cos{(x)}^{ 5 }}  \cos{(x)}^{6 }}} = \int \frac{1}{\tan{(x)}^{ 5/3 }} d(\tan{(x)}) = \frac{\tan{(x)}^{ -2/3 }}{-\dfrac{2}{3}} + C 
}$$

$$\displaylines{
\int \frac{dx}{4 \cdot  3\sin{(x)} + 4\cos{(x)}} = \begin{vmatrix}
t = \tan{\left( \dfrac{x}{2} \right)}  & \sin{(x)} = \dfrac{2t}{t^{ 2 } + 1} \\
x = 2\arctan{(t)} & \cos{(x)} = \dfrac{1 - t^{ 2 }}{1+t^{ 2 }} \\
dx =  \dfrac{2dt}{1+t^{ 2 }}
\end{vmatrix} = \int \dfrac{\dfrac{2dt}{1+t^{ 2 }}}{4 \cdot  3 \cdot \dfrac{2t}{1+t^{ 2 }} + 4 \cdot \dfrac{1-t^{ 2 }}{1+t^{ 2 }} } = \int \frac{2dt}{-4(t^{ 2 }-6t-1)} = -\frac{1}{4\sqrt{ 10 }}\ln\left| \frac{\tan{\left( \dfrac{x}{2} \right)}-3-\sqrt{ 10 }}{\tan{\left( \dfrac{x}{2} \right)}-3+\sqrt{ 10 }} \right| + C
}$$

$$\displaylines{
\int \cos{(5x)}^{ 4 }dx = \int  \left( \frac{1+\cos{(10x)}}{2}  \right)^{ 2 }dx = \frac{1}{4} \int 1+2\cos{(10x)} + \frac{1+\cos{(20x)}}{2} dx = \frac{1}{4}\int \left( \frac{3}{2} + 2\cos{(10x)} + \frac{1}{2} \cos{(20x)} \right)dx = \frac{1}{4}\left( \frac{3}{2}dx + 2 \frac{1}{10} \sin{(10x)} + \frac{1}{2} \frac{1}{20} \sin{(20x)} \right) + C
}$$

$$\displaylines{
\int \frac{1+\sqrt{ x }}{\sqrt[3]{ x } + 2} dx = \begin{vmatrix}
t = \sqrt[6]{ x }  \\
x = t^{ 6 } \\
dx = 6t^{ 5 }dt
\end{vmatrix} = \int \left( \frac{1+t^{ 3 }}{t^{ 2 } + 2} \cdot  6t^{ 5 } \right)dt =6 \int \left( t^6 - 2t^4 + t^3 + 4t^2 - 2t - 8 + \frac{4t + 16}{t^2 + 2} \right) dt =6 \left( \frac{t^7}{7} - \frac{2t^5}{5} + \frac{t^4}{4} + \frac{4t^3}{3} - t^2 - 8t + 2\ln(t^2 + 2) + \frac{16}{\sqrt{2}} \arctan\left(\frac{t}{\sqrt{2}}\right) \right) + С
}$$

$$\displaylines{
\int \frac{dx}{\sqrt[4]{ x^{ 3 } } ( \sqrt[8]{ x } - 1)^{ 5 }} = \int { x^{ -3/4 } } ( \sqrt[8]{ x } - 1)^{ -5 } = \begin{vmatrix}
p = -5 \\
n = \dfrac{1}{8} \\
m = -\dfrac{3}{4}
\end{vmatrix} = \begin{vmatrix}
t = x^{ 1/8 } \\
x = t^{ 8 } \\
x^{ -3/4 } = t^{ -6 } \\
dx = 8t^{ 7 }dt
\end{vmatrix}= \dots 
}$$

$$\displaylines{
\int \arccos{(2x)}dx = x\arccos{(2x)} - \frac{1}{2} \sqrt{ 1 - 4x^{ 2 } } + C
}$$
$$\displaylines{
\int \frac{xdx}{x^{ 2 } + 2x + 10x} = \int \frac{\frac{1}{2}(2x+2)dx}{x^{ 2 } + 2 x + 10} = \frac{1}{2} \ln(x^{ 2 } + 2x + 10) - \frac{1}{3} \arctan{\left( \frac{x+1}{3}  \right)} + C 
}$$

$$\displaylines{
\int (x-1) \ln(x) dx = \frac{1}{2} \frac{x^{ 2 }}{2} - x + \frac{1}{2} \ln|x|
}$$

#### Определенный интеграл.
Основная формула:
$$\displaylines{
\int_{ a }^{ b } f(x)dx = F(x) \bigg|_{ a }^{ b }= F(b) - F(a) 
}$$
$$\displaylines{
\int _{ 2 }^{ 9 } \sqrt[3]{ x-1 } dx = \frac{(x-1)^{ 4/3 }}{4/3} \bigg|_{ 2 }^{ 9 } = \frac{3}{4}(8 ^{ 4/3 } - 1 ^{  4/3 }) = \frac{45}{4}
}$$

Общие методы. Разложение.
Схема:
$$\displaylines{
\int _{ a }^{ b } f(x) dx = \int _{ a }^{ b } [\alpha_{ 1 }g_{ 1 }(x) + \alpha_{ 2 } g_{ 2 }(x) + \dots ]dx
}$$

Пример.
$$\displaylines{
\int_{ 3 }^{ 4 } \frac{x^{ 2 }+3}{x-2}dx = \int_{ 3 }^{ 4 } \left(  x+2  + \frac{7}{x-2} \right)dx = \left( \frac{x^{ 2 }}{2} + 2x + 7\ln|x-2| \right) \bigg|_{ 3 }^{ 4 }  
}$$