$$\displaylines{
q = 5, \  n = 7, \  n_{1}\leq 2, \ n_{2}+n_{3}+n_{4} = 3. \\
A = \{ a_{1}, \ a_{2}, \ a_{3}, \ a_{4}, \ a_{5} \} \\
\square\square\square\square\square\square\square \\
\begin{cases}
n_{1}+n_{2}+n_{3}+n_{4}+n_{5}=7  \\
n_{2}+n_{3}+n_{4} = 3
\end{cases} \implies  \begin{cases}
n_{1}+n_{5} = 4 \\
n_{2}+n_{3}+n_{4} = 3  \\
n_{1}\leq 2
\end{cases}
}$$
$$\displaylines{
\binom{7}{3} \cdot 3^{ 3 } \cdot \bigg(1+\binom{4}{3} + P(2, \ 2)\bigg)
}$$
$$\displaylines{
\begin{array}{|c|c|}
\hline 
n_{1} & n_{5} &  \\
\hline 
0 & 4 & 1 \\
\hline 
1 & 3 & 4 \\
\hline 
2 & 2 & 6 \\
\hline 

\end{array}
}$$
---
### Рекуррентные соотношения порядка второго порядка.
$$\displaylines{
x_{n} = d_{ 1 }x_{n-1} + d_{ 2 } x_{n-2} \\
\lambda^{ 2 } = d_{ 1 }\lambda + d_{ 2 } \\
\lambda^{ 2 }-d_{1}\lambda-d_{2} = 0 \\
1) \ \lambda_{ 1 } - \lambda_{ 2 } = \lambda^{ *n }(\text{ кратный корень }) \implies  \exists C_{ 1 }, \ C_{ 2 }:x_{n} = \lambda^{ *n }(C_{ 1 }+C_{ 2 }n) \\
(\lambda-\lambda^{ * }) = 0 \\
2) \lambda_{ 1 }\neq \lambda_{ 2 } \implies  \exists C_{ 1 }, \ C_{ 2 }: x_{n} = C_{ 1 }\lambda_{ 1 }^{ n }+C_{ 2 }\lambda_{2}^{ n }
}$$
Пример. 
$$\displaylines{
x_{n+2} = 5x_{n+1}-6x_{n}, \ x_{ 1 } = 1, \ x_{2} = 2 \\
\lambda^{ 2 }=5\lambda-6 \\
\lambda_{ 1 } = 3, \  \lambda_{ 2 } = 2 \\
(\lambda-3)(\lambda-2) = 0 \\
x_{n} = C_{ 1 }\lambda_{ 1 }^{ n } + C_{ 2 } \lambda^{ n }_{ 2 } = C_{ 1 }3^{ n } + C_{ 2 }2^{ n } = \frac{1}{2}\cdot 2^{ n }=2^{ n-1 }\\
\begin{cases}
x_{ 0 } = 3C_{ 1 }+2C_{ 2 } = 1 \\
x_{ 1 } = 9\cdot C_{ 1 } + 4C_{ 2 } = 2 
\end{cases}\implies \begin{cases}
C_{ 1 } = 0  \\
C_{ 2 } = \dfrac{1}{2} 
\end{cases}
}$$
Пример.
$$\displaylines{
x_{n+2} = 2x_{n+1} - x_{n}, \ x_{ 0 }=1, \ x_{ 1 } = 6 \\
\lambda^{ 2 } = 2\lambda-1 \\
\lambda_{ 1, \ 2 } = 1 \\
x_{n} = \lambda^{ n }(C_{ 1 }+C_{ 2 }) \\
x_{ 0 } = C_{ 1 } = 1 \\
x_{ 1 } = C_{ 1 } + C_{ 2 } = 6, \ C_{ 2 } = 5 \\
x_{n}=1+5n
}$$
Пример.
$$\displaylines{
A_{ n+2 } = 3A_{ n+1 } - 2A_{ n } \quad A_{ 0 } = 1 \quad A_{ 1 } = 1 \\
\lambda^{ 2 } = 3\lambda-2 \quad \lambda^{ 2 }-3\lambda+2 = 0 \quad \lambda_{ 1 } = 1, \  \lambda_{ 2 } = 2 \\
A_{ n } = \lambda^{ n }_{ 1 }C_{ 1 } + \lambda_{ 2 }^{ n } C_{ 2 } \\
A_{ 0 } = C_{ 1 } + C_{ 2 } = 1 \\
A_{ 1 } = 1 C_{ 1 } + 2C_{2} =1 \\
C_{ 2 }=0, \ C_{ 1 } = 1 \\
A_{ n } = 1^{ n }\cdot 1 + 2^{ n } \cdot  0  = 1 
} $$
Пример.
$$\displaylines{
a_{n+2} = a_{ n+1 } + a_{n}, \  a_{ 0 } = 1, \ a_{1} = 1 \\
\lambda^{ 2 }=\lambda+1 \\
\lambda_{ 1, \ 2 } = \frac{1\pm \sqrt{ 5 }}{2} \\
a_{ 0 } = C_{ 1 } \cdot  \lambda_{ 1 }^{ n } + C_{ 2 }\cdot \lambda_{ 2 }^{ n } \\
\begin{cases}
1 = C_{ 1 } + C_{ 2 }  \\
1 = C_{ 1 } \cdot  \dfrac{1-\sqrt{ 5 }}{2} + C_{ 2 } \cdot  \dfrac{1+\sqrt{ 5 }}{2} 
\end{cases} \\
\text{Матрица коэффициентов:} \begin{vmatrix} 1 & 1 \\ \frac{1-\sqrt{5}}{2} & \frac{1+\sqrt{5}}{2} \end{vmatrix} \\
D = \det\begin{vmatrix} 1 & 1 \\ \frac{1-\sqrt{5}}{2} & \frac{1+\sqrt{5}}{2} \end{vmatrix} = 1 \cdot \frac{1+\sqrt{5}}{2} - 1 \cdot \frac{1-\sqrt{5}}{2} = \frac{1+\sqrt{5}}{2} - \frac{1-\sqrt{5}}{2} = \sqrt{5}. \\

D_1 = \det\begin{vmatrix} 1 & 1 \\ 1 & \frac{1+\sqrt{5}}{2} \end{vmatrix} = 1 \cdot \frac{1+\sqrt{5}}{2} - 1 \cdot 1 = \frac{1+\sqrt{5}}{2} - 1 = \frac{-1+\sqrt{5}}{2}. \\
C_1 = \frac{D_1}{D} = \frac{\frac{-1+\sqrt{5}}{2}}{\sqrt{5}} = \frac{-1+\sqrt{5}}{2\sqrt{5}} = \frac{-1}{2\sqrt{5}} + \frac{\sqrt{5}}{2\sqrt{5}} = \frac{-1 + \sqrt{5}}{10}. \\
\\
D_2 = \det\begin{vmatrix} 1 & 1 \\ \frac{1-\sqrt{5}}{2} & 1 \end{vmatrix} = 1 \cdot 1 - 1 \cdot \frac{1-\sqrt{5}}{2} = 1 - \frac{1-\sqrt{5}}{2} = \frac{2 - (1 - \sqrt{5})}{2} = \frac{1 + \sqrt{5}}{2}. \\
C_2 = \frac{D_2}{D} = \frac{\frac{1+\sqrt{5}}{2}}{\sqrt{5}} = \frac{1+\sqrt{5}}{2\sqrt{5}} = \frac{1}{2\sqrt{5}} + \frac{\sqrt{5}}{2\sqrt{5}} = \frac{1 + \sqrt{5}}{10}.
}$$
$$\displaylines{
a_{n} =\frac{-1 + \sqrt{5}}{10} \cdot \left( \frac{1-\sqrt{ 5 }}{2}  \right)^{ n } +  \frac{1 + \sqrt{5}}{10}\cdot \left( \frac{1+\sqrt{ 5 }}{2}  \right)^{ n }
}$$
