# Exercise 1 
$$\displaylines{
z = i = 0 + 1i \\ 
r = \sqrt{ 0 + 1^{2} } = 1 \\ 
\tan \phi = \frac{1}{0} \implies \phi = \frac{\pi}{2} \\ 
z = 1 \cdot \left( \cos \frac{\pi}{2} + i \sin \frac{\pi}{2} \right) \\
z^{ \frac{1}{3} } = 1^{ \frac{1}{3} } \cdot \left( \cos \frac{\frac{\pi}{2} + 2\pi k}{3} + i \sin \frac{\frac{\pi}{2} + 2\pi k}{3} \right) \\ 
k = 0 \implies z^{ \frac{1}{3} } = \cos \frac{\pi}{6} + i \sin \frac{\pi}{6} = \frac{\sqrt{ 3 }}{2} + \frac{1}{2} i  \\ 
k = 1 \implies z^{ \frac{1}{3} } = \cos \frac{5\pi}{6} + i \sin \frac{5\pi}{6} = \frac{\sqrt{ 3 }}{2} - \frac{1}{2} i \\ 
k = 2 \implies z^{ \frac{1}{3} } = \cos \frac{3\pi}{2} + i \sin \frac{3\pi}{2} = 0 - 1i = -1i \\ 
}$$

# Exercise 2 
$$\displaylines{
z = \cos \frac{\pi}{2} + i\sin \frac{\pi}{2} \\ 
z^{ \frac{1}{6} } = 1^{ \frac{1}{6} } \cdot \left( \cos \frac{\frac{\pi}{2} + 2\pi k}{6} + i \sin \frac{\frac{\pi}{2} + 2\pi k}{6} \right) = \cos \frac{\frac{\pi}{2} + 2\pi k}{6} + i \sin \frac{\frac{\pi}{2} + 2\pi k}{6} \\ 
k = 0 \implies z^{ \frac{1}{6} } = \cos \frac{\pi}{12} + i \sin \frac{\pi}{12} = \frac{1 + \sqrt{ 3 }}{2 \sqrt{ 2 }} + i \frac{\sqrt{ 3 } - 1}{2 \sqrt{ 2 }} \\ 
k = 1 \implies z^{ \frac{1}{6} } = \dots 
}$$

# Exercise 3 
$$\displaylines{
z = -4 + 0i \\ 
r = 4 \\ 
\tan \phi = \frac{0}{-4} = 0 \implies \phi = \pi \\ 
z = 4 \cdot (\cos \pi + i \sin \pi) \\ 
z^{ \frac{1}{4} } = \sqrt{ 2 } \cdot \left( \cos \frac{\pi + 2\pi k}{4} + i \sin \frac{\pi + 2\pi k}{4} \right) \\ 
k = 0 \implies z^{ \frac{1}{4} } = \sqrt{ 2 } \cdot \left( \cos \frac{\pi}{4} + i \sin \frac{\pi}{4} \right) = \sqrt{ 2 } \cdot \left( \frac{\sqrt{ 2 }}{2} + i \frac{\sqrt{ 2 }}{2} \right) = 1 + i \\ 
k = 1 \implies z^{ \frac{1}{4} } = \sqrt{ 2 } \cdot \left( \cos \frac{3\pi}{4} + i \sin \frac{3\pi}{4} \right) = \sqrt{ 2 } \cdot \left( \frac{\sqrt{ 2 }}{2} - i \sin \frac{\sqrt{ 2 }}{2} \right) = 1 - i \\ 
k = 2 \implies z^{ \frac{1}{4} } = \dots 
}$$

# Exercise 4 
$$\displaylines{
z = 1 + i \\ 
r = \sqrt{ 2 } \\ 
\tan \phi = \frac{1}{1} \implies \phi = \frac{\pi}{4} \\ 
z = \sqrt{ 2 } \cdot \left( \cos \frac{\pi}{4} + i \sin \frac{\pi}{4} \right) \\ 
z^{ \frac{1}{3} } = \sqrt[6]{ 2 } \cdot \left( \cos \frac{\frac{\pi}{4} + 2 \pi k}{3} + i \sin \frac{\frac{\pi}{4} + 2 \pi k}{3} \right) \\ 
k = 0 \implies z^{ \frac{1}{3} } = \dots 
}$$