# Exercise 4.1 
## Exercise 1 
$$\displaylines{
(1 - i) \cdot (2 + 3i) = (1 \cdot 2 + 1 \cdot 3) + i(1 \cdot 3 - 1 \cdot 2) = 5 + i 
}$$

## Exercise 3
$$\displaylines{
\text{Re}((2 - i) \cdot (1 + i)) \\ 
(2 - i) \cdot (1 + i) = (2 + 1) + i(2 - 1) = 3 + i \\ 
\text{Re}(3  + i) = 3
}$$

## Exercise 7 
$$\displaylines{
(1 + i) \cdot \overline{(2 - 3i) \cdot (1 - i)} = (1 + i) \cdot \overline{(2 - 3) + i(-2 -3)} = (1 + i) \cdot \overline{-1 -5i} = \\ (1 + i) \cdot (-1 + 5i) = (-1 - 5) + i(5 - 1) = -6 + 4i
}$$

# Exercise 4.2 
## Exercise 1
$$\displaylines{
\frac{1 + 2i}{1 - i} = \frac{1 + 2i}{1 - i} \cdot \frac{1 + i}{1 + i} = \frac{(1 - 2) + i(1 + 2)}{2} = \frac{-1 + 3i}{2} = -\frac{1}{2} + \frac{3}{2} i
}$$

## Exercise 4
$$\displaylines{
\text{Re}\left( \frac{1 - 2i}{2 - i} \right) = \text{Re}\left( \frac{4}{5} - \frac{3}{5}i \right) = \frac{4}{5} \\ 
\frac{1 - 2i}{2 - i} = \frac{1 - 2i}{2 - i} \cdot \frac{2 + i}{2 + i} = \frac{(2 + 2) + i(1 - 4)}{5} = \frac{4 - 3i}{5} = \frac{4}{5} - \frac{3}{5}i
}$$

## Exercise 7
$$\displaylines{
\text{Im}\left( \frac{(1 + 2i)^{2}}{(1 - i)^{ 3 }} \right) = \\
\frac{(1 + 2i)^{ 2 }}{(1 - i)^{ 3 }} = \frac{1 + 4i - 4}{1 - 3i + 3i^{2} - i^{ 3 }} = \frac{-3 + 4i}{-2 - 2i} = \\
= \frac{-3 + 4i}{-2 - 2i} \cdot \frac{-2 + 2i}{-2 + 2i} = \frac{(6 - 8) + i(-6-8)}{8} = \frac{-2 + -14i}{8} = -\frac{1}{4} - \frac{7}{4}i
}$$

# Exercise 4.5 
## Exercise 1 


## Exercise 2

# Exercise 4.7 
## Exercise 1
$$\displaylines{
(5 - 8i)x + (7 + 3i)y = 2 - i \\ 
5x - i(8x) + 7y + i(3y) = 2 - i \\ 
\begin{cases} 
5x + 7y = 2 \\
-8x + 3y = -1 
\end{cases} \\ 
x = \frac{13}{71} \\ 
y = \frac{11}{71}
}$$

## Exercise 3
$$\displaylines{
(5 + 2i)x + (6 - 5i)y = -2 + 3i \\ 
5x + i(2x) + 6y - i(5y) = -2 + 3i \\ 
\begin{cases}
5x + 6y = - 2 \\
2x - 5y = 3 
\end{cases} \\ 
x = \frac{8}{37} \\
y = - \frac{19}{37}
}$$
# Exercise 4.9 
## Exercise 1 
$$\displaylines{
z \cdot \overline{z} + z = 22 + 4i \\ 
a^{2} + b^{2} + (a + bi) = 22 + 4i \\ 
\begin{cases}
a^{2} + a + b^{2} = 22 \\
b = 4
\end{cases} \\ 
a^{2} + a + 16 = 22 \\ 
a^{2} + a - 6 = 0 \\ 
a_{ 1 } = - 3 \implies z_{ 1 } = -3 + 4i \\ 
a_{ 2 } = 2 \implies z_{ 2 } = 2 + 4i 
}$$

## Exercise 3 
$$\displaylines{
z \cdot \overline{z} + \overline{z} = 7 - i \\ 
a^{2} + b^{2} + (a - bi) = 7 - i \\ 
\begin{cases}
a^{2} + a + b^{2} = 7 \\
b = 1 
\end{cases} \\ 
a^{2} + a - 6 = 0 \\ 
a_{ 1 } = -3 \implies z_{ 1 } = -3 + i \\ 
a_{ 2 } = 2 \implies z_{ 2 } = 2 + i
}$$