
Определение. ${\displaystyle x_{0}}$ - корень ${\displaystyle f(x)}$, если ${\displaystyle f(x_{0}) = 0}$.
${\displaystyle x_{0}}$ - корень кратности ${\displaystyle s}$, если ${\displaystyle f(x_{0}) = 0, \ f'(x_{0}) = 0, \ f^{ (s-1) }(x_{0}) = 0, \ \dots, \ f^{ (s) }(x_{0}) \neq0}$.

Утверждение. ${\displaystyle x_{0}}$ - корень  кратности ${\displaystyle s}$, если ${\displaystyle f(x) \ \vdots \ (x-x_{0})^{ s }}$.

Пусть корни ${\displaystyle f(x)}$ - это ${\displaystyle a_{1}, \ \dots, \ a_{n}}$. А соответствующие им кратности - ${\displaystyle s_{ 1 }, \ \dots , \ s_{ n }}$.
Тогда многочлен можно записать так:
$$\displaylines{
f(x) = (x - a_1)^{s_1} \cdot (x - a_2)^{s_2} \cdot \dots \cdot (x - a_n)^{s_n}.\\
f'(x) = s_1 (x - a_1)^{s_1 - 1} \cdot (x - a_2)^{s_2} \cdot \dots \cdot (x - a_n)^{s_n} + \dots + s_n (x - a_1)^{s_1} \cdot \dots \cdot (x - a_{n-1})^{s_{n-1}} \cdot (x - a_n)^{s_n - 1}.
}$$

$$\displaylines{
f(x) = x^{ 5 } - x^{ 4 } - 2x^{ 3} + 2x^{ 2 } + x-1 \ | \ \cdot 5 \\
f'(x) = 5x^{ 4 } -4x^{ 3 } - 6x^{ 2 } + 4x + 1 \\

}$$