# Part 1 
**Exercise 1:**
$$\displaylines{
x_{ n } = \frac{6}{n} + 1
}$$

**Exercise 2:**
$$\displaylines{
x_{ n } = n^{2} - 2
}$$

**Exercise 3:**
$$\displaylines{
x_{ n } = (-1)^{ n } \cdot n
}$$

# Part 2 
**Exercise 1:** Prove that the sequence is limited. 
$$\displaylines{
x_{ n } = (-1)^{ n } \cdot 4 + 3 \\ 
|x_{ n }| = |(-1)^{ n } \cdot 4 + 3| \leq |(-1)^{ n } \cdot 4| + |3| = 4 + 3 = 7 \\ 
|x_{ n }| \leq 7
}$$

**Exercise 2:** Prove that the sequence is limited. 
$$\displaylines{
x_{ n } = 4\cos 2n - 3 \sin 4n + 1 \\ 
|x_{ n }| = |4\cos 2n - 3 \sin 4n + 1| \leq |4\cos 2n| + |-3\sin 4n| + |1| \leq 4 + 3 + 1 = 8 \\ 
|x_{ n }| \leq 8
}$$

**Paragraph 7, Exercise 275:** Prove that the sequences are limited. 
$$\displaylines{
x_{ n } = \frac{2n ^{2}  - 1}{2 + n^{2}} \\ 
|x_{ n }| = | \frac{2n^{2} - 1}{2 + n^{2}} | = \frac{2n^{2} - 1}{2 + n^{2}} \leq \frac{2n^{2} + 4}{n^{2} + 2} = 2 \\ 
|x_{ n }| \leq 2
}$$
$$\displaylines{
x_{ n } = \frac{1 - n}{\sqrt{ n^{2} + 1 }} \\ 
|x_{ n }| = | \frac{1 - n}{\sqrt{ n^{2} + 1 }} | \leq \frac{n - 1}{\sqrt{ n^{2} + 1 }} \leq \frac{n + 0}{\sqrt{ n^{2} + 0 }} = \frac{n}{\sqrt{ n^{2} }} = \frac{n}{n} = 1 \\ 
|x_{ n }| \leq 1 
}$$
$$\displaylines{
x_{ n } = \frac{n^{2} + 4n + 8}{(n + 1)^{2}} \\ 
|x_{ n }| = | \frac{n^{2} + 4n + 8}{(n + 1)^{2}} | = \frac{n^{2} + 4n + 8}{(n + 1)^{2}} = \frac{n^{2} + 2n + 1 + 2n + 7}{(n + 1)^{2}} = 1 + \frac{2n + 7}{(n + 1)^{2}} \leq 1 + \frac{n^{2} + 2n + 7}{(n + 1)^{2}} = 2 + \frac{6}{(n + 1)^{2}} \\ 
\begin{cases}
|x_{ n }| \leq 2 + \frac{6}{(n + 1)^{2}}  \\
\max \left( 2 + \frac{6}{(n + 1)^{2}} \right) = 2 + \frac{6}{4} = 3.5 
\end{cases} \implies |x_{ n }| \leq 4
}$$

**Paragraph 7, Exercise 276:** Prove that the sequences are limited. 
$$\displaylines{
x_{ n } = (-1)^{ n } \cdot n \\ 
|x_{ n }| = |(-1)^{ n } \cdot n| = n \\ 
n > c \implies n(c) = [c] + 1
}$$
$$\displaylines{
x_{ n } = n^{2} - n \\ 
|x_{ n }| = |n^{2} - n| \geq n^{2} - n \geq n \\ 
n > c \implies n(c) = [c] + 1
}$$
$$\displaylines{
| \frac{n^{ 3 }}{n^{2} + 1}|= \frac{n^{ 3 }}{n^{2} + 1} \geq \frac{n^{ 3 }}{n^{ 2 } + n^{2}} = \frac{n}{2} \\ 
\frac{n}{2} > c \\
n > 2c \\ 
n(c) = [2c] + 1
}$$



