Продифференцировать используя формулы первого уровня.
$$\displaylines{
a) \ y = 3x + 5x^{ 2 } - \frac{7}{x} + 8 \\ 
y' = 3+ 10x +\frac{7}{x^{ 2 }}
}$$
$$\displaylines{
б) \ y = 9-3\sqrt{ x }+\sqrt[3]{ 8x^{ 2 } } \\
y' = -3 \cdot \frac{1}{2}x^{ -1/2 }((8x^{ 2 })^{ 1/3 })' = -1, \ 5 \cdot \frac{1}{\sqrt{ x }} + 2\cdot \frac{2}{3}x^{ -1/3 } = -1,5 \cdot \frac{1}{\sqrt{ x }}+\frac{4}{3\sqrt[3]{ x }}
}$$
$$\displaylines{
в) \ y = 2 - 3 \frac{2}{x^{ 2 }\sqrt{ x }} + \ln(\cos{(e^{ \sin{(6)} })}) \\
y = 2- \frac{6}{x^{ 5/2 }} + \dots  \\
y' = 0 + \frac{15}{x^{ 7/2 }} +0
}$$
$$\displaylines{
г) \ y = \frac{2x-\ln(4)\sqrt{ x } - 6x\sqrt[6]{ x^{ 5 } }}{ \cos{(5)} \cdot  x\sqrt[3]{ x } } \\
= \frac{2}{\cos{(5)}} \cdot x^{ -1/3 } - \frac{\ln(4)}{\cos{(5)}}\cdot x^{ 1/2-4/3 } - \frac{6}{\cos{(5)}}\cdot x^{ 11/6-4/3 } \\
y' = -\frac{2}{\cos{(5)}\cdot 3} \cdot  x^{ -4/3 } + \frac{5\ln(4)}{6\cos{(5)}}\cdot x^{ -11/6 } - \frac{6}{2\cos{(5)}}\cdot x^{ -1/2 } 
}$$
$$\displaylines{
д) \ y = \left( \frac{x\sqrt[3]{ x\sqrt{ x } }}{x^{2}}  \right)^{ 3/4 } \\
y = \left( \frac{x\cdot x^{ 1/2 }}{x^{ 2 }}  \right)^{ 3/4 } = (x^{ -1/2 })^{ 3/4 }
= x^{ -3/8 }\\
y' = -\frac{3}{8}\cdot x^{ -11/8 }
}$$
$$\displaylines{
е) \ y = \frac{(\sqrt[3]{ x }-3x\sqrt{ x })^{ 2 }}{\sqrt{ x\sqrt{ x } }} = \frac{\sqrt[3]{ x^{ 2 } } -2\sqrt[3]{ x }\cdot 3x\sqrt{ x }+4x^{ 2 }x}{x^{ 1/2 }\cdot x^{ 1/4 }} = \frac{x^{ 2/3 } - 6x^{ 1/3 } \cdot  x \cdot  x^{ 1/2 }+9x^{ 3 }}{x^{ 3/4 }} = (x^{ 2/3 }-6x^{ 11/6}+9x^{ 3 })\cdot x^{ -3/4 } = \\
= -x^{ 2/3-3/4 } - 6x^{ 11/6-3/4 } +9x^{ 3-3/4 } = x^{ -1/12 } - 6x^{ 13/12 } + 9x^{ 9/4 } \\
y' = -\frac{1}{12}x^{ -13/12 } - \frac{13}{2}x^{ 1/12 } + \frac{81}{4}x^{ 5/4 }
}$$
$$\displaylines{
ж) \ y = \frac{(\sqrt[3]{ x }+2\sqrt{ x })^{ 2 }}{3x(2x\sqrt[3]{ x^{ 4 } })^{ 2 }} \\
}$$
$$\displaylines{
з) \ y = \frac{(2x - \sqrt{ x })^{ 3 }}{\sqrt{ x\sqrt[3]{ 16x } }} 
}$$
---
1. Записать функции
	a) $f(x) = \cos(x)$, $g(x) = \ln(x)$, $h(x) = x^{4}$

1. Композиция $f \circ g \circ h (x)$:
$$
\displaylines{
(f \circ g \circ h)(x) = \cos(\ln(x^{4})) = \cos(4 \ln x)
}
$$

2. Композиция $h \circ g \circ h \circ f (x)$:
$$
\displaylines{
(h \circ g \circ h \circ f)(x) = (4 \ln(\cos x))^{4}
}
$$

3. Композиция $g \circ h \circ f (x)$:
$$
\displaylines{
(g \circ h \circ f)(x) = 4 \ln(\cos x)
}
$$

	b) $f(x) = \cot(x)$, $g(x) = e^{x}$, $h(x) = x^{2}$

1. Композиция $f \circ g \circ h (x)$:
$$
\displaylines{
(f \circ g \circ h)(x) = \cot(e^{x^{2}})
}
$$

2. Композиция $h \circ g \circ h \circ f (x)$:
$$
\displaylines{
(h \circ g \circ h \circ f)(x) = e^{2 (\cot x)^{2}}
}
$$

3. Композиция $g \circ h \circ f (x)$:
$$
\displaylines{
(g \circ h \circ f)(x) = e^{(\cot x)^{2}}
}
$$

	c) $f(x) = \log_{2}(x)$, $g(x) = x^{3/2}$, $h(x) = 2^{2x}$

1. Композиция $f \circ g \circ h (x)$:
$$
\displaylines{
(f \circ g \circ h)(x) = 3x
}
$$

2. Композиция $h \circ g \circ h \circ f (x)$:
$$
\displaylines{
(h \circ g \circ h \circ f)(x) = 2^{2x^{3}}
}
$$

3. Композиция $g \circ h \circ f (x)$:
$$
\displaylines{
(g \circ h \circ f)(x) = x^{3}
}
$$
---

2. Представить в виде композиции ${f(x) = \sin{(x)}, \ g(x) = \ln(x), \ h(x) = x^{ 3 }}$ функции:
	a) $[\sin(\ln(x))]^{3}$:
$$
\displaylines{
h(f(g(x)))
}
$$

	b) $\ln(\sin(x^{3}))$:
$$
\displaylines{
g(f(h(x)))
}
$$

	c) $\ln([\ln(\sin(x))^{3}]^{3})$:
$$
\displaylines{
g(h(g(h(f(x)))))
}
$$

	d) $\sin([\sin(\ln(x))]^{3})$:
$$
\displaylines{
f(h(f(g(x))))
}
$$
---
3. Записать 
	1. ${f = g(x)}$
	2. ${g \circ f(x)}$
	если
		a) ${f(x) = 2x+ \tan{(x)}^{ 2 }}$, ${g(x) = \sin{(x + x^{ 3 })}}$
		б) ${f(x) = 2\tan{(x)}^{ 2 }+ x\sqrt{ \ln(x) }}$, ${g(x) = \frac{x}{\arcsin{(x)}}}$

a) $f(x) = 2x + \tan^{2}(x)$, $g(x) = \sin(x + x^{3})$

1. Композиция $f \circ g(x)$:
$$
\displaylines{
(f \circ g)(x) = f(g(x)) = 2\,\sin(x + x^{3}) + \tan^{2}\big(\sin(x + x^{3})\big)
}
$$

2. Композиция $g \circ f(x)$:
$$
\displaylines{
(g \circ f)(x) = g(f(x)) = \sin\big(f(x) + [f(x)]^{3}\big) = \sin\big(2x + \tan^{2}(x) + (2x + \tan^{2}(x))^{3}\big)
}
$$

b) $f(x) = 2\,\tan^{2}(x) + x\,\sqrt{\ln(x)}$, $g(x) = \frac{x}{\arcsin(x)}$

1. Композиция $f \circ g(x)$:
$$
\displaylines{
(f \circ g)(x) = f(g(x)) = 2\,\tan^{2}\left(\frac{x}{\arcsin(x)}\right) + \frac{x}{\arcsin(x)}\,\sqrt{\ln\left(\frac{x}{\arcsin(x)}\right)}
}
$$

2. Композиция $g \circ f(x)$:
$$
\displaylines{
(g \circ f)(x) = g(f(x)) = \frac{f(x)}{\arcsin(f(x))} = \frac{2\,\tan^{2}(x) + x\,\sqrt{\ln(x)}}{\arcsin\left(2\,\tan^{2}(x) + x\,\sqrt{\ln(x)}\right)}
}
$$
