# Part 1 
**Exercise 58.1:**
$$\displaylines{
\lim_{ n \to \infty } \left( \frac{2002}{n} \right)^{ n } = 0^{ \infty } = 0
}$$

**Exercise 58.2:** 
$$\displaylines{
\lim_{ n \to \infty } \left( \frac{a}{n} \right)^{ n } = 0^{ \infty } = 0
}$$

**Exercise 58.3:** 
$$\displaylines{
\lim_{ n \to \infty } \left( \frac{2n + 3}{n^{2}} \right)^{ n } = 0^{ \infty } = 0
}$$

**Exercise 58.4:**
$$\displaylines{
\lim_{ n \to \infty } \left( \frac{n + 10}{2n - 1} \right)^{ n } = 0^{ \infty } = 0
}$$

**Exercise 61.1:**
$$\displaylines{
\lim_{ n \to \infty } \displaylines{\sqrt[3n]{ 8 }} = \lim_{ n \to \infty } 8^{ \frac{1}{3n} } = 8^{ 0 } = 1
}$$

**Exercise 61.2:** 
$$\displaylines{
\lim_{ n \to \infty } \sqrt[2n]{ \frac{1}{2} } = \lim_{ n \to \infty } \frac{1}{2^{ \frac{1}{2n} }} = \frac{1}{1} = 1
}$$

**Exercise 61.3:** 
$$\displaylines{
\lim_{ n \to \infty } \sqrt[n^{2}]{ 6 } = \lim_{ n \to \infty } 6^{ \frac{1}{n^{2}} } = 1
}$$

**Exercise 61.4:** 
$$\displaylines{
\lim_{ n \to \infty } \frac{\sqrt[n]{ 10 } - 2}{1 + \sqrt[n]{ \frac{1}{100} }} = \lim_{ n \to \infty } \frac{10^{ \frac{1}{n}} - 2}{1 + \frac{1}{100^{ \frac{1}{n} }}} = \frac{1 - 2}{1 + 1} = -\frac{1}{2}
}$$
t
**Exercise 61.5:** 
$$\displaylines{
\lim_{ n \to \infty } \sqrt[n]{ 2 + \frac{1}{n} } = \lim_{ n \to \infty } \left( 2 + \frac{1}{n} \right)^{ \frac{1}{n} } = 2^{ 0 } = 1
}$$

**Exercise 61.6:**
$$\displaylines{
\lim_{ n \to \infty } \sqrt[n]{ \frac{5n + 1}{n + 5} } = \lim_{ n \to \infty }\left( 5 - \frac{24}{n + 5} \right)^{ \frac{1}{n} } = 5^{ 0 } = 1
}$$

**Exercise 61.7:**
$$\displaylines{
\lim_{ n \to \infty } \sqrt[n]{ \frac{2n + 5}{n - \frac{1}{2}} } = \lim_{ n \to \infty } \left( 2 + \frac{6}{n - \frac{1}{2}} \right)^{ \frac{1}{n} } = 2^{ 0 } = 1
}$$

 **Exercise 61.8:**
 $$\displaylines{
\lim_{ n \to \infty } \sqrt[n]{ 3^{ n } + 2^{ n } } = \lim_{ n \to \infty } (3^{ n } + 2^{ n })^{ \frac{1}{n} } = \lim_{ n \to \infty } (3^{ n })^{ \frac{1}{n} } = 3 
}$$

**Exercise 61.9:**
$$\displaylines{
\lim_{ n \to \infty } \frac{\sqrt[n]{ 3 } - 1}{\sqrt[n]{ 9 } - 1} = \lim_{ n \to \infty }  \frac{\sqrt[n]{ 3 } - 1}{(\sqrt[n]{ 3 } - 1) \cdot (\sqrt[n]{ 3 } + 1)} = \lim_{ n \to \infty } \frac{1}{\sqrt[n]{ 3 } + 1} = \frac{1}{2}
}$$

**Exercise 61.10:** 
$$\displaylines{
\begin{aligned}
\lim_{ n \to \infty } \frac{\sqrt[n]{ 8 } - 1}{\sqrt[n]{ 2 } - 1} &= \lim_{ n \to \infty } \frac{\sqrt[n]{ 2 }^{ 3 } - 1}{\sqrt[n]{ 2 } - 1} \\ 
&= \lim_{ n \to \infty } \frac{(\sqrt[n]{ 2 } - 1) \cdot (\sqrt[n]{ 4 } + \sqrt[n]{ 2 } + 1)}{\sqrt[n]{ 2 } - 1} \\ 
&= \lim_{ n \to \infty } \sqrt[n]{ 4 } + \sqrt[n]{ 2 } + 1 = 1 + 1 + 1 = 3
\end{aligned}
}$$

**Exercise 61.11:** 
$$\displaylines{
\lim_{ n \to \infty } 4^{ \frac{n + 2}{n + 1} } = \lim_{ n \to \infty } 4^{ 1 + \frac{1}{n + 1} } = 4^{ 1 } = 4
}$$

**Exercise 61.12:** 
$$\displaylines{
\lim_{ n \to \infty } (1 + 11^{ n })^{ \frac{1}{n + 2} } = \lim_{ n \to \infty } \left( 11^{ n } \cdot \left( \frac{1}{11^{ n } } + 1\right) \right)^{ \frac{1}{n + 2} } = \lim_{ n \to \infty } (11^{ n })^{ \frac{1}{n + 2} } = \lim_{ n \to \infty } 11^{ \frac{n}{n + 2} } = 11^{ 1 } = 11 
}$$

**Exercise 64.1:** 
$$\displaylines{
\lim_{ n \to \infty } \frac{n^{ 3 } + 3^{ n }}{n + 3^{ n + 1 }} = \lim_{ n \to \infty } \frac{n^{ 3 } + 3^{ n }}{n + 3 \cdot 3^{ n }} = \lim_{ n \to \infty } \frac{3^{ n }}{3 \cdot 3^{ n }} = \frac{1}{3}
}$$

**Exercise 64.2:** 
$$\displaylines{
\lim_{ n \to \infty } \frac{n^{ 10 } - 1}{1 + n \cdot 1.1^{ n }} = 0
}$$

**Exercise 64.3:**
$$\displaylines{
\begin{aligned}
\lim_{ n \to \infty } \sqrt[n]{ 3^{ n } + n \cdot 2^{ n } } &= \lim_{ n \to \infty } \sqrt[n]{ 3^{ n } \cdot \left( 1 + \frac{n \cdot 2^{ n }}{3^{ n }} \right) }  \\
&= \lim_{ n \to \infty } \sqrt[n]{ 3^{ n } } = 3
\end{aligned}
}$$

**Exercise 66.1:** 
$$\displaylines{
\lim_{ n \to \infty } \frac{n \cdot \lg(n)}{n^{2} - 1} = 0
}$$

**Exercise 66.2:**
$$\displaylines{
\lim_{ n \to \infty } \frac{5n + \lg(n)}{n - 3.5} = \lim_{ n \to \infty } \frac{5n}{n} = 5
}$$

**Exercise 66.3:** 
$$\displaylines{
\lim_{ n \to \infty } \frac{\log_{2}(n + 3)}{n - 1.3} = \lim_{ n \to \infty } \frac{\log_{2}\left( n \cdot \left( 1 + \frac{3}{n} \right) \right)}{n \cdot \left( 1 - \frac{1.3}{n} \right)} = \lim_{ n \to \infty } \frac{\log_{2}(n) + \log_{2}\left( 1 + \frac{3}{n} \right)}{n \cdot \left( 1 - \frac{1.3}{n} \right)} = \lim_{ n \to \infty } \frac{\log_{2}(n)}{n} = 0
}$$

**Exercise 66.4:**
$$\displaylines{
\lim_{ n \to \infty } \frac{\log_{5}(n^{2} + 1)}{n} = \lim_{ n \to \infty } \frac{\log_{5}\left( n^{2} \cdot \left( 1 + \frac{1}{n^{2}} \right) \right)}{n} = \lim_{ n \to \infty } \frac{\log_{5}(n^{2}) + \log_{5}\left( \frac{1}{n^{2}} \right)}{n} = \lim_{ n \to \infty } \frac{2 \cdot \log_{5}(n)}{n} = 0
}$$

**Exercise 66.5:**
$$\displaylines{
\lim_{ n \to \infty } \frac{n - \lg(n)}{\log_{2}(4^{ n } + 1)} = \lim_{ n \to \infty } \frac{n \cdot \left( 1 - \frac{\lg(n)}{n} \right)}{2n} = \lim_{ n \to \infty } \frac{n}{2n} = \frac{1}{2}
}$$

**Exercise 68.1:**
$$\displaylines{
\lim_{ n \to \infty } \frac{(-2)^{ n }}{(n + 2)!} = 0
}$$

**Exercise 68.2:**
$$\displaylines{
\lim_{ n \to \infty } \frac{1}{(0.3)^{ n } \cdot n!} = 0
}$$

**Exercise 68.3:**
$$\displaylines{
\lim_{ n \to \infty } \frac{n \cdot 3^{ n } + 1}{n! + 1} = \lim_{ n \to \infty } \frac{n \cdot 3^{ n }}{n \cdot (n - 1)!} = \lim_{ n \to \infty } \frac{3^{ n }}{(n - 1)!} = 0
}$$

**Exercise 68.4:**
$$\displaylines{
\lim_{ n \to \infty } \frac{4^{ n } + n^{2} \cdot 2^{ n } - 1}{n^{ 4 } + (n!)^{2}} = \lim_{ n \to \infty } \frac{4^{ n }}{(n!)^{2}} = 0
}$$

**Exercise 68.5:**
$$\displaylines{
\lim_{ n \to \infty } \frac{10^{ n } + n!}{2^{ n } + (n + 1)!} = \lim_{ n \to \infty } \frac{10^{ n }}{(n + 1)!} = 0
}$$

# Part 2
**Exercise 1:**
$$\displaylines{
\lim_{ n \to \infty } \frac{2^{ n } + n}{n! + 3} = \lim_{ n \to \infty } \frac{2^{ n }}{n!} = 0
}$$

**Exercise 2:**
$$\displaylines{
\lim_{ n \to \infty } \frac{3^{ n } + n^{2}}{2n + 3^{ n + 2 }} = \lim_{ n \to \infty } \frac{3^{ n }}{3^{ n + 2 }} = \lim_{ n \to \infty } \frac{3^{ n }}{9 \cdot 3^{ n }} = \frac{1}{9}
}$$

**Exercise 3:**
$$\displaylines{
\lim_{ n \to \infty } \frac{2n^{ n } + 3 \cdot n^{ 122 } + 9^{ n }}{100n + n^{ n }} = \lim_{ n \to \infty } \frac{2n^{ n }}{n^{ n }} = 2
}$$

**Exercise 4:**
$$\displaylines{
\lim_{ n \to \infty } \frac{2n - 16^{ n + 2 } + 3^{ n }}{4^{ 2n + 3 } - 100n^{ 100 } - 256^{ \frac{n}{2} + 1 }} = \lim_{ n \to \infty } \frac{-16^{ n + 2 }}{4^{ 2n + 3 } - 256^{ \frac{n}{2} + 1 }} = \lim_{ n \to \infty } \frac{-16^{2} \cdot 2^{ 4n }}{4^{ 3 } \cdot 2^{ 4n } - 256 \cdot 2^{ 4n }} = \frac{-2^{ 8 }}{2^{ 6 } - 2^{ 8 }} = -\frac{4}{3}
}$$

**Exercise 5:**
$$\displaylines{
\lim_{ n \to \infty } \frac{25^{ \frac{n}{2} } - (n + 2)!}{n^{2} \cdot (3^{ n -1 } - n + n!)} = \lim_{ n \to \infty } \frac{5^{ n } - (n + 2)!}{n^{2} \cdot 3^{ n - 1 } - n^{ 3 } + n^{2} \cdot n!} = \lim_{ n \to \infty } \frac{-(n + 2)!}{n^{2} \cdot n!} = \\
= \lim_{ n \to \infty } \frac{-n! \cdot (n + 1) \cdot (n + 2)}{n^{2} + n!} = \lim_{ n \to \infty } \frac{(n + 1) \cdot (n+ 2)}{n^{2}} = \lim_{ n \to \infty } \frac{n^{2} + 3n + 2}{n^{2}} = \lim_{ n \to \infty } \frac{n^{2}}{n^{2}} = 1
}$$

**Exercise 6:**
$$\displaylines{
\lim_{ n \to \infty } \frac{n \cdot n^{ n } + 2n!}{n! + 3n^{ n + 1 }} = \lim_{ n \to \infty } \frac{n \cdot n^{ n }}{3n^{ n + 1 }} = \lim_{ n \to \infty } \frac{n^{ n + 1 }}{3n^{ n + 1 }} = \frac{1}{3}
}$$

**Exercise 7:**
$$\displaylines{
\lim_{ n \to \infty } \frac{\left( \frac{3}{2} \right)^{ n } + 3n^{ 100 }}{3 + \frac{9}{2} + \frac{27}{4} + \dots + \frac{3^{ n }}{2^{ n - 1 }}} = \lim_{ n \to \infty } \frac{ \left( \frac{3}{2} \right)^{ n } }{\frac{3^{ n }}{\frac{2^{ n }}{2}}} = \lim_{ n \to \infty } \frac{\left( \frac{3}{2} \right)^{ n }}{2 \cdot \left( \frac{3}{2} \right)^{ n }} = \frac{1}{2}
}$$

**Exercise 8:**
$$\displaylines{
\lim_{ n \to \infty } \sqrt{ 9^{ n } - 2 \cdot 3^{ n } } - \sqrt{ 9^{ n } + 2^{ n } } = \lim_{ n \to \infty } \frac{9^{ n } - 2 \cdot 3^{ n } - 9^{ n } - 2^{ n }}{\sqrt{ 9^{ n } - 2 \cdot 3^{ n } } + \sqrt{ 9^{ n } + 2^{ n } }} = \lim_{ n \to \infty } \frac{-2 \cdot 3^{ n } - 2^{ n }}{\sqrt{ 9^{ n } } + \sqrt{ 9^{ n } }} = \lim_{ n \to \infty } \frac{-2 \cdot 3^{ n }}{2 \cdot 3^{ n }} = -1
}$$

# Part 3
**Formula:** 
$$\displaylines{
\lim_{ n \to \infty } \left( 1 + \frac{1}{n} \right)^{ n } = \lim_{ n \to \infty } (1 + n)^{ \frac{1}{n} } = e
}$$

**Exercise 1:**
$$\displaylines{
\begin{aligned}
\lim_{ n \to \infty } \left( 1 + \frac{3}{n + 3} \right)^{ 2n - 1 } &= \lim_{ n \to \infty } \left( 1 + \frac{1}{\frac{n + 3}{3}} \right)^{ 2n - 1 } \\ 
&= \lim_{ n \to \infty } \left(\left( 1 + \frac{1}{\frac{n + 3}{3}} \right)^{ \frac{n + 3}{3} }\right)^{ \frac{3}{n + 1} \cdot (2n - 1) } \\ 
&= \lim_{ n \to \infty } e^{ \frac{3 \cdot (2n - 1)}{n + 1} } \\ 
&= \lim_{ n \to \infty } e^{ \frac{6n}{n} } = e^{ 6 }
\end{aligned}
}$$

**Exercise 2:**
$$\displaylines{
\begin{aligned}
\lim_{ n \to \infty } \left( 1 + \frac{2n}{5n^{2} + 1} \right)^{ \frac{n^{ 4 } + 2}{(n + 1) \cdot (n^{2} + 3)} } &= \lim_{ n \to \infty } \left( \left( 1 + \frac{1}{\frac{5n^{2} + 1}{2n}} \right)^{ \frac{5n^{2} + 1}{2n} } \right)^{ \frac{2n}{5n^{2} + 1} \cdot \frac{n^{ 4 } + 2}{(n + 1) \cdot (n^{2} + 3)} } \\ 
&= \lim_{ n \to \infty } e^{ \frac{2n \cdot (n^{ 4 } + 2)}{(5n^{2} + 1) \cdot (n + 1) \cdot (n^{2} + 3)} } \\
&= \lim_{ n \to \infty } e^{ \frac{2n^{ 5 }}{5n^{ 5 }} } = e^{ \frac{2}{5} }
\end{aligned} 
}$$

**Exercise 3:**
$$\displaylines{
\lim_{ n \to \infty } \left( 1 + \frac{n}{2^{ n } + n} \right)^{ \frac{4^{ \frac{n}{2} } + 1}{2n + 3\ln(n)} } \\ 
\dots
}$$

**Exercise 4:** 
$$\displaylines{
\lim_{ n \to \infty } \left( \frac{n^{2} + 2}{n^{2} + 1} \right)^{ 2n^{2} } = \lim_{ n \to \infty } \left( 1 + \frac{1}{n^{2} + 1} \right)^{ 2n^{2} } \\ 
\dots
}$$

**Exercise 5:** 
$$\displaylines{
\begin{aligned}
\lim_{ n \to \infty } \left( \frac{2n^{ 3 } + 3n}{2n^{ 3 } + 1} \right)^{ -n^{2} } &= \lim_{ n \to \infty } \left( \frac{2n^{ 3 } + 1 + 3n}{2n^{ 3 } + 1} \right)^{ -n^{2} } \\ 
&= \lim_{ n \to \infty } \left( 1 + \frac{3n}{2n^{ 3 } + 1} \right)^{ -n^{2} } \\ 
&= \lim_{ n \to \infty } \left( 1 + \frac{1}{\frac{2n^{ 3 } + 1}{3n}} \right)^{ -n^{2} } \\ 
&= \lim_{ n \to \infty } \left( \left( 1 + \frac{1}{\frac{2n^{ 3 } + 1}{3n}} \right)^{ \frac{2n^{ 3 } + 1}{3n} } \right)^{ \frac{3n}{2n^{ 3 } + 1} \cdot (-n^{2}) } \\ 
&= \lim_{ n \to \infty } e^{ -\frac{3n^{ 3 }}{2n^{ 3 } + 1} } = e^{ -\frac{3}{2} }
\end{aligned}
}$$




