# Complex Numbers 
**Exercise 5.5.1:**
$$\displaylines{
|z| + z = 8 + 4i \\ 
z = a + bi \\ 
\sqrt{ a^{2} + b^{2} } + a + bi = 8 + 4i \\ 
\begin{cases}
\sqrt{ a^{2} + b^{2} } + a = 8 \\
b = 4
\end{cases}
\sqrt{ a^{2} + 16 } + a = 8 \\ 
\sqrt{ a^{2} + 16 } = 8 - a \\ 
a^{2} + 16 = 64 - 16a + a^{2} \\ 
16a = 64 - 16 \\ 
a = 4 - 1 = 3 \\ 
z = 3 + 4i 
}$$

**Exercise 5.5.2:**
$$\displaylines{
|z| - z = 2 - 4i \\ 
z = a + bi \\
\sqrt{ a^{2} + b^{2} } - a - bi = 2 - 4i \\
\begin{cases}
\sqrt{ a^{2} + b^{2} } - a = 2 \\
-b = -4 \implies b = 4
\end{cases} \\ 
\sqrt{ a^{2} + 16 } = a + 2 \\ 
a^{2} + 16 = a^{2} + 4a + 4 \\ 
4a = 16 - 4 = 12 \\ 
a = 3 \\ 
z = 3 + 4i
}$$

**Exercise:**
$$\displaylines{
|z| + i\overline{z} = 1 - 5i \\ 
z = a + bi \\ 
\sqrt{ a^{2} + b^{2} } + i(a - bi) = 1 - 5i\\ 
\sqrt{ a^{2} + b^{2} } + ai + b = 1 - 5i \\ 
\begin{cases}
\sqrt{ a^{2} + b^{2} } + b = 1  \\
a = -5 \implies a = 5
\end{cases} \\ 
\sqrt{ b^{2} + 25 } = 1 - b \\
b^{2} + 25 = 1 - 2b + b^{2} \\ 
2b = -24 \\ 
b = -12 
}$$

**Exercise:**
$$\displaylines{
|z| = z^{2} \\ 
z = a + bi \\
\sqrt{ a^{2} + b^{2} } = (a + bi)^{2} = a^{2} + 2abi - b^{2} \\ 
\sqrt{ a^{2} + b^{2} } = a^{2} + 2abi - b^{2} \\ 
\begin{cases}
\sqrt{ a^{2} + b^{2} } = a^{2} - b^{2}  \\
2ab = 0 
\end{cases} \\ 
2ab = 0 \implies \begin{matrix}a = 0 \\ b = 0\end{matrix} \\ 
a =  0 \implies \sqrt{ b^{2} } = - b^{2} \implies b = 0 \\
b = 0 \implies \sqrt{ a^{2} } = a^{2} \implies a = 0, 1, -1 \\ 
z_{ 1 } = 0 \\ 
z_{ 2 } = 1 \\ 
z_{ 3 } = -1
}$$

**Exercise:**
$$\displaylines{
\arg z = \frac{\pi}{4} \\ 
}$$

**Exercise:**
$$\displaylines{
\arg z^{2} = \frac{\pi}{3} \\ 
\arg z = \phi \\ 
\arg z^{2} = 2\phi + 2\pi k, \ \ k \in \mathbb{Z} \\ 
2 \phi = \frac{\pi}{3} + 2\pi \\ 
\phi = \frac{\pi}{6} + \pi 
}$$

**Exercise:**
$$\displaylines{
\overline{z} = \left( \frac{1}{2} + i \frac{\sqrt{ 3 }}{2} \right) \cdot z \\ 
\frac{1}{2} + i\frac{\sqrt{ 3 }}{2} = \cos \frac{\pi}{3}  + i\sin \frac{\pi}{3} \\ 
z = r \cdot (\cos \phi + i\sin \phi) \\ 
(!) \ \ r \cdot (\cos -\phi + i \sin \phi) = \left( \cos \frac{\pi}{3} + i \sin \frac{\pi}{3} \right) \cdot r \cdot (\cos \phi + i \sin \phi) \\ 
-\phi = \frac{\pi}{3} + \phi + 2\pi k \\ 
-2\phi = \frac{\pi}{3} + 2\pi k \\ 
\phi = -\frac{\pi}{6} + \pi k  \\ 
k = 0 \implies -\frac{\pi}{6} \text{ or } \frac{11\pi}{6} \text{ because } 0 \leq \phi \leq 2\pi \\ 
k = 1 \implies \frac{5\pi}{6} 
}$$

**Exercise:**
$$\displaylines{
\cos (3 \phi) \\ 
(\cos \phi + i \sin \phi)^{ 3 } = \cos (3\phi) + i\sin(3\phi) \\ 
(\cos \phi + i \sin \phi)^{ 3 } = \cos^{ 3 } \phi + 3 \cdot  \cos^{2}\phi \cdot i\sin \phi - 3 \cdot \cos \phi \cdot \sin^{ 2 } \phi - i\sin^{ 3 } \phi \\ 
\cos (3\phi) = \cos^{ 3 } - 3\cos \phi \cdot \sin^{2} \phi \\ 
\sin (3\phi) = 3 \cos^{2} \phi \sin \phi - \sin^{ 3 }\phi
}$$

**Exercise:**
$$\displaylines{
\cos^{ 3 }x = \\ 
\begin{matrix}
z + \frac{1}{z} = 2 \cdot \cos \phi \text{ if } z = \cos \phi + i \sin \phi \\ 
z^{ -1 } + z = \overline{z} + z \\ 
\frac{1}{z^{2}} + z^{2} = 2 \cos (2 \phi) \\ 
\end{matrix} \implies \frac{1}{z^{ n }} + z^{ n } = 2 \cos (n\phi) \\ 
\cos \phi = \frac{1}{2} \cdot \left( \frac{1}{z} + z \right) \\ 
\begin{aligned}
\cos^{ 3 } \phi &= \frac{1}{8} \cdot \left( \frac{1}{z} + z \right)^{ 3 } \\
&= \frac{1}{8} \cdot \left( \frac{1}{z^{ 3 }} + 3 \cdot \frac{1}{z^{2}} \cdot z + 3 \cdot \frac{1}{z} \cdot z^{2} + z^{3}  \right) \\ 
&= \frac{1}{8} \cdot \left( \frac{1}{z^{ 3 }} + 3 \cdot \frac{1}{z} + 3 \cdot z + z^{3}  \right) \\ 
&= \frac{1}{8} \cdot \left( \left( \frac{1}{z^{ 3 }} + z^{ 3 } \right) + 3 \cdot \left( \frac{1}{z} + z \right) \right) \\
&= \frac{1}{8} (2 \cos 3 \phi + 6 \cos \phi)
\end{aligned}
}$$

**Exercise:**
$$\displaylines{
\begin{aligned}
\cos^{ 4 } \phi &= \frac{1}{16} \cdot \left( \frac{1}{z} + z \right)^{ 4 } \\
&= \frac{1}{16} \cdot \left( \left( \frac{1}{z^{ 4 }} +  z^{ 4 } \right) + 4 \cdot \left( \frac{1}{z^{ 2 }} + z^{2} \right) + 6 \right) \\
=& \frac{1}{16} \cdot (2 \cos 4\phi + 8 \cos 2\phi + 6)
\end{aligned}
}$$

**Exercise:**
$$\displaylines{
\sin^{ 3 } \phi  = \text{?} \\ 
z - \frac{1}{z} = (\cos \phi + i \sin \phi) - \cos \phi + i \sin \phi = 2i\sin \phi \implies \\
\implies \sin \phi = \frac{1}{2i} \cdot \left( z - \frac{1}{z} \right) \\ 
\begin{aligned}
\sin^{ 3 } \phi &= - \frac{1}{8i} \cdot \left( z^{ 3 } - 3 \cdot z^{2} \cdot \frac{1}{z} + 3 \cdot z \cdot \frac{1}{z^{2}} - \frac{1}{z^{ 3 }} \right) \\ 
&= - \frac{1}{8i} \cdot \left( z^{ 3 } - \frac{1}{z^{ 3 }}  - 3 \cdot \left( z - \frac{1}{z} \right) \right) \\ 
&= \dots \\ 
&= \frac{1}{4} \cdot \sin 3 \phi + \frac{3}{4} \cdot \sin \phi 
\end{aligned}
}$$

# Systems 
**Exercise:**
$$\displaylines{
5x_{ 1 } + 5x_{ 2 } + 5x_{ 3 } + 12x_{ 4 } = 10 \\ 
2x_{ 1 } + 2x_{ 2 } + 3x_{ 3 } + 5x_{ 4 } = 4 \\ 
x_{ 1 } + 7x_{ 2 } + 9x_{ 3 } + 4x_{ 4 } = 2 \\ 
\begin{pmatrix}
5 & 3 & 5 & 12 & \mid 10 \\
2 & 2 & 3 & 5 & \mid 4 \\
1 & 7 & 9 & 4 & \mid 2
\end{pmatrix} \implies 
\begin{pmatrix}
5 & 3 & 5 & 12 & \mid 10 \\
0 & -12 & -15 & -3 & \mid 0 \\
1 & 7 & 9 & 4 & \mid 2
\end{pmatrix} \implies
\begin{pmatrix}
0 & -32 & -40 & -8 & \mid 0 \\
0 & -12 & -15 & -3 & \mid 0 \\
1 & 7 & 9 & 4 & \mid 2
\end{pmatrix} \implies
\begin{pmatrix}
0 & 4 & 5 & 1 & \mid 0 \\
0 & 4 & 5 & 1 & \mid 0 \\
1 & 7 & 9 & 4 & \mid 2
\end{pmatrix} \implies \\ 
\implies \begin{pmatrix}
0 & 0 & 0 & 0 & \mid 0 \\
0 & 4 & 5 & 1 & \mid 0 \\
1 & 7 & 9 & 4 & \mid 2
\end{pmatrix} \\ 
\begin{cases}
x_{ 1 } + 7x_{ 2 } = 2 - 9x_{ 3 } - 4x_{ 4 } \\
4x_{ 2 } = 5x_{ 3  } - x_{ 4 }
\end{cases}
}$$
$$\displaylines{
\text{Free: } x_{ 3 }, x_{ 4 } \\ 
\text{Main: } x_{ 1 }, x_{ 2 } \\ 
x_{ 2 } = \frac{-5x_{ 3 } - x_{ 4 }}{4} \\ 
x_{ 1 } + 7 \cdot \left( \frac{-5x_{ 3 } - x_{ 4 }}{4} \right) = 2 - 9x_{ 2 } - 4x_{ 4 } \\ 
\begin{aligned}
x_{ 1 } &= 2 - 9x_{ 3 } - 4x_{ 4 } - 7 \cdot \left( \frac{-5x_{ 3 } - x_{ 4 }}{4} \right) \\ 
&= \frac{8 - 36x_{ 3 } - 16x_{ 4 } + 35x_{ 3 } + 7x_{ 4 }}{4} \\ 
&= \frac{8 - x_{ 3 }  - 9x_{ 4 }}{4}
\end{aligned} \\ 
x_{ \text{general solution} } = \left( \frac{8 - x_{ 3 } - 9x_{ 4 }}{4}, \frac{-5x_{ 3 } - x_{ 4 }}{4}, x_{ 3 }, x_{ 4 } \right)
}$$

**Exercise:**
$$\displaylines{
\begin{pmatrix} 
-9 & 6 & 7 & 10 & \mid 3 \\
-6 & 4 & 2 & 3 & \mid 2 \\
-3 & 2 & -11 & -15 & \mid 1
\end{pmatrix} \implies 
\begin{pmatrix} 
0 & 0 & 40 & 55 & \mid 0 \\
-6 & 4 & 2 & 3 & \mid 2 \\
-3 & 2 & -11 & -15 & \mid 1
\end{pmatrix} \implies
\begin{pmatrix} 
0 & 0 & 40 & 55 & \mid 0 \\
0 & 0 & 24 & 33 & \mid 0 \\
-3 & 2 & -11 & -15 & \mid 1
\end{pmatrix} \implies \\ 
\implies \begin{pmatrix} 
0 & 0 & 8 & 11 & \mid 0 \\
0 & 0 & 8 & 11 & \mid 0 \\
-3 & 2 & -11 & -15 & \mid 1
\end{pmatrix} \implies
\begin{pmatrix} 
0 & 0 & 8 & 11 & \mid 0 \\
-3 & 2 & -11 & -15 & \mid 1
\end{pmatrix}
}$$
$$\displaylines{
\begin{cases}
8x_{ 3 } + 11x_{ 4 } = 0 \\
-3x_{ 1 } + 2x_{ 2 } - 11x_{ 3 } - 15x_{ 4 } = 1  
\end{cases} \implies 
\begin{cases}
x_{ 3 } = - \frac{11x_{ 4 }}{8} \\
15x_{ 4 } = -3x_{ 1 } 
\end{cases}
}$$

**Homework:** 
Complex Numbers: 5.25 8) 9); 5.14 4)

System: 
$$\displaylines{
\begin{cases}
-9x_{ 1 } + 10x_{ 2 } + 3x_{ 3 } + 7x_{ 4 } = 7  \\
-4x_{ 1 } + 7x_{ 2 } + x_{ 3 } + 3x_{ 4 } = 5 \\
7x_{ 1 } + 5x_{ 2 } - 4x_{ 3 } - 6x_{ 4 } = 3
\end{cases} \\ 
}$$
