$$\displaylines{
f \cancel{\in } T_{ 0 } \cup  T_{ 1 } \cup  S, \  f - \text{ Шефферова } \iff  [\{ f \}] = P_{ 2 }
}$$
Доказательство:
1. ${\displaystyle f \cancel{ \in } T_{ 0 }, \ f \cancel{ \in} T_{ 1 }, \ f \cancel{ \in} S}$
$$\displaylines{
f(0, \  0, \  \dots , \  0) = 1, \ f(1, \  \dots , \  1) = 0, \   \implies  f \cancel{ \in } M
}$$
2. От противного. Пусть ${\displaystyle f \in L }$, то есть функция представима в виде
$$\displaylines{
f = \alpha_{ 0 } \oplus x_{1} \oplus  \alpha_{ 2 }x_{2}\oplus  \dots \oplus \alpha_{ n }x_{n} \\
f(0, \  \dots , \  0) = 1 \implies  \alpha_{ 0 } = 1
}$$
Проверим ${\displaystyle \overline{f}(x) = f(\overline{x})}$.
$$\displaylines{
f(1, \  \dots , \  1) = 0 \\
f = 1 \oplus  \alpha_{ 1 } \oplus \alpha_{2} \oplus  \dots \oplus \alpha_{ n } = 0 \\
\alpha_{ 1 } \oplus \alpha_{2} \oplus  \dots \oplus \alpha_{ n } = 1
f(\overline{x}) = 1 \oplus  \alpha_{1}(x_{1}\oplus 1) \oplus  \alpha_{2}(x_{2}\oplus 1) \oplus \dots \oplus  \alpha_{ n }(x_{n} \oplus 1) = \\
= 1 \oplus  \alpha_{ 1 } \oplus \alpha_{2} \oplus  \dots \oplus \alpha_{ n } \oplus \alpha_{ 1 } x_{1} \oplus  \alpha_{ 2 }x_{2} \oplus \dots \oplus \alpha_{ n }x_{n} = \\= \alpha_{ 1 } x_{1} \oplus  \alpha_{ 2 }x_{2} \oplus \dots \oplus \alpha_{ n }x_{n} \\
\overline{f} = 1 \oplus  1 \oplus  \alpha_{ 1 } x_{1} \oplus  \alpha_{ 2 }x_{2} \oplus \dots \oplus \alpha_{ n }x_{n}
}$$
Равны.

${\displaystyle A}$ - базис, если:
1. ${\displaystyle [A] = P_{ 2 }}$, ${\displaystyle A}$ - полная система.
2. ${\displaystyle \forall{f} \in A: [A\backslash\{ f \}] \neq P_{ 2 } }$
Базис содержит не более 4 функций.

$$
|T_0 \cup T_1 \cup S| = 2^{2^n - 1} + 2^{2^n - 1} + 2^{2^{n-1}} - 2^{2^n - 2} - 2^{2^{n-1} - 1} - 2^{2^{n-1} - 1} + 2^{2^{n-1} - 1}
$$
$$
= 2^{2^n} - 2^{2^n - 2} + 2^{2^{n-1}} - 2^{2^{n-1} - 1}
$$
$$
|P_2(n) - (T_0 \cup T_1 \cup S)| = 2^{2^n} - (2^{2^n} - 2^{2^n - 2} + 2^{2^{n-1}} - 2^{2^{n-1} - 1})
$$
$$
= 2^{2^n - 2} - 2^{2^{n-1}} + 2^{2^{n-1} - 1}
$$
