$$\displaylines{
x \to  y = \overline{x} \vee y \\x \downarrow y = \overline{x \vee y} \\
x \oplus  y = x \overline{y} \vee \overline{x} y \\
x \sim y =  xy \vee \overline{x} \ \overline{ y} \\
\overline{x \vee y} = \overline{x} \wedge \overline{y} \\
\overline{x} = x \oplus 1 \\
x \vee xy = x \\
x \wedge (x \vee y) x \\
x \vee \overline{x} y = x \vee y \\
x \wedge (\overline{x} \vee y) = x y 
}$$

5.6
$$\displaylines{
f(x_{1}, \  x_{2}) = (x_{2} \to  x_{1}) (x_{2} \downarrow  x_{2}) = (\overline{x}_{ 2 } \vee x_{1}) (\overline{x_{2} \vee x_{2}}) = (\overline{x_{2}} \vee x_{ 1 }) \overline{x_{2}} \ \overline{x_{2}} = \\
= (\overline{x_{2}} \vee x_{1}) \overline{x_{2}} = x_{1} \overline{x_{2}} \vee \overline{x_{2}} = \overline{x_{2}}
} $$
$$\displaylines{
f(x_{1}, \  x_{2}, \  x_{3}) = ((x_{1} \oplus x_{2}) \to  x_{3}) (\overline{x_{3}} \to  x_{2}) = (\overline{(x_{1} \overline{x_{2}} \vee \overline{x_{1}}x_{2})} \vee x_{3}) (\overline{\overline{x_{3}} \vee x_{2}}) = \\
= (\overline{x_{1} \overline{x_{2}}} \ \overline{\overline{x_{1}} x_{2}} \vee x_{3}) \overline{\overline{x_{3}}} \ \overline{x_{2}} = ((\overline{x_{1}} \vee x_{2})(x_{1} \vee \overline x_{2}) \vee x_{3}) \cdot  x_{3} \overline{x_{2}} = \\
= (x_{1} \overline{x_{1}} \vee \overline{x_{1}} \ \overline{x_{2}} \vee x_{1} x_{2} \vee x_{2} \overline{x_{2}} \vee x_{3}) \cdot  \overline{x_{2}} x_{3} = \\
= \dots = \overline{x_{2}} x_{3}
}$$
5.10
$$\displaylines{ 
f_{ 1 } = x_{1} \vee x_{2} \vee x_{3}, \   f_{ 2 } = x_{1} \oplus x_{2} \oplus x_{3}\\
\begin{array}{|c|c|}
\hline 
x_{1} & x_{2} & x_{3} & f_{ 1 } & f_{ 2 } \\
\hline 
0 & 0 & 0 & 0  & 0\\
0 & 0 & 1 &  1 & 1\\
0 & 1 & 0  &  1 & 1 \\
0 & 1 & 1 &  1 & 0\\
1 & 0 & 0 & 1  & 1\\
1 & 0 & 1 &  1 & 0\\
1 & 1 & 0 & 1  & 0\\
1 & 1 & 1  & 1 & 1\\
\hline 
\end{array} \\
f_{ 1 } \neq f_{ 2 }
}$$
$$\displaylines{
f_{ 1 } = x_{1} \downarrow (x_{2} \downarrow x_{3}) \\
f_{ 2 } = (x_{1} \downarrow x_{2}) \downarrow x_{3} 
}$$
![[Pasted image 20250328154612.png]]
${\displaystyle f_{ 1 } \neq f_{ 2 }}$

5.6.10