график модуль x

Например, функция ${y = |x|}$, не дифференцируема в ${0}$, но ${x = 0}$ - точка минимума.

график 21:14

$$\displaylines{
x_{ 0 } - \text{ т. min } f(x), \ \text{ если } \\
\exists \ \varepsilon >0 : \forall{x \in U_{ \varepsilon } (x_{ 0 }) \hookrightarrow f(x_{ 0 })} \leq  f(x) \\
x_{ 0 } - \text{ т. max } f(x), \ \text{ если } \\
\exists \varepsilon >0 : \forall{x \in U_{ \varepsilon }} (x_{ 0 }) \hookrightarrow f(x_{ 0 }) \geq f(x) 
}$$

Рассмотрим ${f(x) = \sqrt[3]{ x }, \ x \in \mathbb{R}}$ 
$$\displaylines{
f'(x) = \frac{1}{3x^{ 2/3 }} = 0 \\

}$$
прямая +0+
при ${x \to 0 \quad f'(x) \to + \infty}$, вертикальная касательная в точке ${0}$

$$\displaylines{
f''(x) = \left( \frac{1}{3} x^{ -2/3 } \right)' = -\frac{2}{9x^{ 5/3 }} = 0 \\
}$$
прямая +0- 

при ${x \to 0 \quad f''(x) \to \infty}$ - ${ 0 }$ - точка перегиба

график функции ${\sqrt[3]{ x^{ 2 } }e^{ x }, \ x \in \mathbb{R}}$, ${f(0) = 0, \quad f(x)>0}$
$$\displaylines{
y' = (x^{ 2/3 }e^{ x })' = \frac{2}{3}x^{ -1/3 } e^{ x } + x^{ 2/3 } e^{ x } = e^{ x }\left( \frac{2}{3x^{ 1/3 }} + x^{ 2/3 } \right) = 0 \\
\frac{2 + 3x}{3x^{ 1/3 }} = 0 \\
}$$
прямая  + -2/3 - 0 + 


$$\displaylines{
y'' = \left( e^{ x } \frac{2+3x}{3x^{ 1/3 }}  \right)' = e^{ x } \frac{2+3x}{3x^{ 1/3 }} + e^{ x } \frac{3 \cdot  3x^{ 1/3 } - (2+3x)x^{ -2/3 }}{9x^{ 2/3 }} =   e^{ x } \left(\frac{2+3x}{3x^{ 1/3 }} + \frac{3 \cdot  3x^{ 1/3 } - (2+3x)x^{ -2/3 }}{9x^{ 2/3 }} \right) = \\
 = e^{ x } \frac{(2+3x)3x^{ 1/3 } + 3 \cdot  3x^{ 1/3 } - (2+3x)x^{ -2/3 }  \ |\cdot x^{ 2/3 }}{9x^{ 2/3 } \ |\cdot x^{ 2/3 }} = e^{ x } \frac{(2+3x)3x + 3 \cdot  3x - (2+3x) \cdot  1}{9x^{ 4/3 }}  = \\
 = e^{ x } \frac{ 9x^{ 2 } + 6x + 9x - 2 - 3x}{9x^{ 4/3 }} = e^{ x } \frac{9x^{ 2 } + 12x - 2}{9x^{ 4/3 }} = 0 \\
 \\
 9x^{ 2 } + 12x-2  =0 \\
 x_{ 1,2 } = \frac{-2 \pm \sqrt{ 6 }}{3} = \ \bigg[ \begin{matrix}
\sim 0,16 \\
\sim -1,5
\end{matrix}
}$$
прямая +--+

точки перегиба: ${x = \frac{-2 \pm \sqrt{ 6 }}{3}}$ 

график функции ${\sqrt[3]{ x^{ 2 } }e^{ x }}$


\section*{Полезно}
график

$$\displaylines{
\begin{matrix}
y = x^{ a }, \ a>1 \\
y' = ax^{ a-1 } \\
y'' = a(a-1)x^{ a-2 } >0 , \  a>1, \ x>0
\end{matrix} \implies y - \text{ вогнута }
}$$
$$\displaylines{
\begin{matrix}
y = x^{ a }, \ 0<a<1 \\ 
y' = ax^{ a-1 } \\
y'' = a(a-1)x^{ a-1 } < 0
\end{matrix} \implies y - \text{ выпукла }
}$$
пример 2. ${ y = \sqrt[3]{ (x+3)(6-x)^{ 2 } }, \ x \in\mathbb{R}}$
$$\displaylines{
y = 0, \ \text{ при } x = -3 \text{ и при  } x = 6 \\
прямая -3 + 6 + \\
y' = ((x+3)^{ 1/6 } (x-6)^{ 2/3 })' = \frac{1}{3} (x+3)^{ -2/3 } (x-6)^{ 2/3 } + (x+3)^{ 1/3 } \cdot \frac{2}{3}(x-6)^{ -1/3 } = \\ = \frac{(x-6)^{ 2/3 }}{3(x+3)^{ 2/3 }} + \frac{2(x+3)^{ 1/3 }}{3(x-6)^{ 1/3 }} = \frac{ (x-6)+2(x+3)}{3(x+3)^{ 2/3 }(x-6)^{ 1/3 }} = \frac{3x}{3(x+3)^{ 2/3 } ( x-6)^{ 1/3 }} = 0     
}$$
прямая  + -3 + 0 - 6 + 

$$\displaylines{
x_{ \min }  = 6, \quad x_{ \max } = 0 \hookrightarrow f(6) = 0; f(0) = \sqrt[3]{ 108 } \approx 4.76\\
y'' = \left( \frac{x}{(x+3)^{ 2/3 }(x-6)^{ 1/3 }}  \right)' = \dots = \frac{-18}{(x-6)^{ 4/3 }(x+3)^{ 5/3 }}= 0 


}$$
прямая + -3 - 6 -
${x = -3}$ - точка перегиба


